simmodsem definition & sim_ctx proof update

ems/SimModSem.v
@@ -36,256 +36,131 @@ Section SIM.
           {R_src R_tgt} (RR: st_local -> st_local -> R_src -> R_tgt -> Prop)
     : bool -> bool -> world -> st_local * itree Es R_src -> st_local * itree Es R_tgt -> Prop :=
   | sim_itree_ret
-      i_src0 i_tgt0 w0 st_src0 st_tgt0
+      f_src f_tgt w0 st_src st_tgt
       v_src v_tgt
-      (RET: RR st_src0 st_tgt0 v_src v_tgt)
+      (RET: RR st_src st_tgt v_src v_tgt)
     :
-      _sim_itree sim_itree RR i_src0 i_tgt0 w0 (st_src0, Ret v_src) (st_tgt0, Ret v_tgt)
+      _sim_itree sim_itree RR f_src f_tgt w0 (st_src, Ret v_src) (st_tgt, Ret v_tgt)
 
   | sim_itree_call
-      i_src0 i_tgt0 w w0 st_src0 st_tgt0
+      f_src f_tgt w w0 st_src st_tgt
       fn varg k_src k_tgt
-      (WF: wf w0 (st_src0, st_tgt0))
-      (K: forall w1 vret st_src1 st_tgt1 (WLE: le w0 w1) (WF: wf w1 (st_src1, st_tgt1)),
-          sim_itree _ _ RR true true w (st_src1, k_src vret) (st_tgt1, k_tgt vret))
+      (WF: wf w0 (st_src, st_tgt))
+      (K: forall w1 vret st_src0 st_tgt0 (WLE: le w0 w1) (WF: wf w1 (st_src0, st_tgt0)),
+          _sim_itree sim_itree RR true true w (st_src0, k_src vret) (st_tgt0, k_tgt vret))
     :
-      _sim_itree sim_itree RR i_src0 i_tgt0 w (st_src0, trigger (Call fn varg) >>= k_src)
-                 (st_tgt0, trigger (Call fn varg) >>= k_tgt)
+      _sim_itree sim_itree RR f_src f_tgt w (st_src, trigger (Call fn varg) >>= k_src)
+                 (st_tgt, trigger (Call fn varg) >>= k_tgt)
 
   | sim_itree_syscall
-      i_src0 i_tgt0 w0 st_src0 st_tgt0
+      f_src f_tgt w0 st_src st_tgt
       fn varg rvs k_src k_tgt
       (K: forall vret,
-          sim_itree _ _ RR true true w0 (st_src0, k_src vret) (st_tgt0, k_tgt vret))
+          _sim_itree sim_itree RR true true w0 (st_src, k_src vret) (st_tgt, k_tgt vret))
     :
-      _sim_itree sim_itree RR i_src0 i_tgt0 w0 (st_src0, trigger (Syscall fn varg rvs) >>= k_src)
-                 (st_tgt0, trigger (Syscall fn varg rvs) >>= k_tgt)
+      _sim_itree sim_itree RR f_src f_tgt w0 (st_src, trigger (Syscall fn varg rvs) >>= k_src)
+                 (st_tgt, trigger (Syscall fn varg rvs) >>= k_tgt)
 
   | sim_itree_inline_src
-      i_src0 i_tgt0 w st_src st_tgt
+      f_src f_tgt w st_src st_tgt
       f fn varg k_src i_tgt
       (FUN: alist_find fn fl_src = Some f)
-      (* (IN: In (fn, f) fl_src ) *)
-      (K: _sim_itree sim_itree RR true i_tgt0 w (st_src, (f varg) >>= k_src) (st_tgt, i_tgt))
+      (K: _sim_itree sim_itree RR true f_tgt w (st_src, (f varg) >>= k_src) (st_tgt, i_tgt))
     :
-      _sim_itree sim_itree RR i_src0 i_tgt0 w (st_src, trigger (Call fn varg) >>= k_src)
+      _sim_itree sim_itree RR f_src f_tgt w (st_src, trigger (Call fn varg) >>= k_src)
                  (st_tgt, i_tgt)
 
   | sim_itree_inline_tgt
-      i_src0 i_tgt0 w st_src st_tgt
+      f_src f_tgt w st_src st_tgt
       f fn varg i_src k_tgt
       (FUN: alist_find fn fl_tgt = Some f)
-      (* (IN: In (fn, f) fl_tgt ) *)
-      (K: _sim_itree sim_itree RR i_src0 true w (st_src, i_src) (st_tgt, (f varg) >>= k_tgt))
+      (K: _sim_itree sim_itree RR f_src true w (st_src, i_src) (st_tgt, (f varg) >>= k_tgt))
     :
-      _sim_itree sim_itree RR i_src0 i_tgt0 w (st_src, i_src)
+      _sim_itree sim_itree RR f_src f_tgt w (st_src, i_src)
                  (st_tgt, trigger (Call fn varg) >>= k_tgt)
 
   | sim_itree_tau_src
-      i_src0 i_tgt0 w0 (st_src0: st_local) (st_tgt0: st_local)
+      f_src f_tgt w0 st_src st_tgt
       i_src i_tgt
-      (K: _sim_itree sim_itree RR true i_tgt0 w0 (st_src0, i_src) (st_tgt0, i_tgt))
+      (K: _sim_itree sim_itree RR true f_tgt w0 (st_src, i_src) (st_tgt, i_tgt))
     :
-      _sim_itree sim_itree RR i_src0 i_tgt0 w0 (st_src0, tau;; i_src) (st_tgt0, i_tgt)
+      _sim_itree sim_itree RR f_src f_tgt w0 (st_src, tau;; i_src) (st_tgt, i_tgt)
 
   | sim_itree_tau_tgt
-      i_src0 i_tgt0 w0 (st_src0: st_local) (st_tgt0: st_local)
+      f_src f_tgt w0 st_src st_tgt
       i_src i_tgt
-      (K: _sim_itree sim_itree RR i_src0 true w0 (st_src0, i_src) (st_tgt0, i_tgt))
+      (K: _sim_itree sim_itree RR f_src true w0 (st_src, i_src) (st_tgt, i_tgt))
     :
-      _sim_itree sim_itree RR i_src0 i_tgt0 w0 (st_src0, i_src) (st_tgt0, tau;; i_tgt)
+      _sim_itree sim_itree RR f_src f_tgt w0 (st_src, i_src) (st_tgt, tau;; i_tgt)
 
   | sim_itree_choose_src
-      i_src0 i_tgt0 w0 (st_src0: st_local) (st_tgt0: st_local)
-      X k_src i_tgt
-      (K: exists (x: X), _sim_itree sim_itree RR true i_tgt0 w0 (st_src0, k_src x) (st_tgt0, i_tgt))
+      f_src f_tgt w0 st_src st_tgt
+      X x k_src i_tgt
+      (K: _sim_itree sim_itree RR true f_tgt w0 (st_src, k_src x) (st_tgt, i_tgt))
     :
-      _sim_itree sim_itree RR i_src0 i_tgt0 w0 (st_src0, trigger (Choose X) >>= k_src)
-                 (st_tgt0, i_tgt)
+      _sim_itree sim_itree RR f_src f_tgt w0 (st_src, trigger (Choose X) >>= k_src)
+                 (st_tgt, i_tgt)
 
   | sim_itree_choose_tgt
-      i_src0 i_tgt0 w0 (st_src0: st_local) (st_tgt0: st_local)
+      f_src f_tgt w0 st_src st_tgt
       X i_src k_tgt
-      (K: forall (x: X), _sim_itree sim_itree RR i_src0 true w0 (st_src0, i_src) (st_tgt0, k_tgt x))
+      (K: forall (x: X), _sim_itree sim_itree RR f_src true w0 (st_src, i_src) (st_tgt, k_tgt x))
     :
-      _sim_itree sim_itree RR i_src0 i_tgt0 w0 (st_src0, i_src)
-                 (st_tgt0, trigger (Choose X) >>= k_tgt)
+      _sim_itree sim_itree RR f_src f_tgt w0 (st_src, i_src)
+                 (st_tgt, trigger (Choose X) >>= k_tgt)
 
   | sim_itree_take_src
-      i_src0 i_tgt0 w0 (st_src0: st_local) (st_tgt0: st_local)
+      f_src f_tgt w0 st_src st_tgt
       X k_src i_tgt
-      (K: forall (x: X), _sim_itree sim_itree RR true i_tgt0 w0 (st_src0, k_src x) (st_tgt0, i_tgt))
+      (K: forall (x: X), _sim_itree sim_itree RR true f_tgt w0 (st_src, k_src x) (st_tgt, i_tgt))
     :
-      _sim_itree sim_itree RR i_src0 i_tgt0 w0 (st_src0, trigger (Take X) >>= k_src)
-                 (st_tgt0, i_tgt)
+      _sim_itree sim_itree RR f_src f_tgt w0 (st_src, trigger (Take X) >>= k_src)
+                 (st_tgt, i_tgt)
 
   | sim_itree_take_tgt
-      i_src0 i_tgt0 w0 (st_src0: st_local) (st_tgt0: st_local)
-      X i_src k_tgt
-      (K: exists (x: X), _sim_itree sim_itree RR i_src0 true w0 (st_src0, i_src) (st_tgt0, k_tgt x))
+      f_src f_tgt w0 st_src st_tgt
+      X x i_src k_tgt
+      (K: _sim_itree sim_itree RR f_src true w0 (st_src, i_src) (st_tgt, k_tgt x))
     :
-      _sim_itree sim_itree RR i_src0 i_tgt0 w0 (st_src0, i_src)
-                 (st_tgt0, trigger (Take X) >>= k_tgt)
+      _sim_itree sim_itree RR f_src f_tgt w0 (st_src, i_src)
+                 (st_tgt, trigger (Take X) >>= k_tgt)
 
   | sim_itree_supdate_src
-      i_src0 i_tgt0 w0 (st_src0: st_local) (st_tgt0: st_local)
+      f_src f_tgt w0 st_src st_tgt
       X k_src i_tgt
       (run: st_local -> st_local * X )
-      (K: _sim_itree sim_itree RR true i_tgt0 w0 (fst (run st_src0), k_src (snd (run st_src0))) (st_tgt0, i_tgt))
+      (K: _sim_itree sim_itree RR true f_tgt w0 (fst (run st_src), k_src (snd (run st_src))) (st_tgt, i_tgt))
     :
-      _sim_itree sim_itree RR i_src0 i_tgt0 w0 (st_src0, trigger (SUpdate run) >>= k_src) (st_tgt0, i_tgt)  
+      _sim_itree sim_itree RR f_src f_tgt w0 (st_src, trigger (SUpdate run) >>= k_src) (st_tgt, i_tgt)  
 
   | sim_itree_supdate_tgt
-      i_src0 i_tgt0 w0 (st_src0: st_local) (st_tgt0: st_local)
+      f_src f_tgt w0 st_src st_tgt
       X i_src k_tgt
       (run: st_local -> st_local * X )
-      (K: _sim_itree sim_itree RR i_src0 true w0 (st_src0, i_src) (fst (run st_tgt0), k_tgt (snd (run st_tgt0))))
+      (K: _sim_itree sim_itree RR f_src true w0 (st_src, i_src) (fst (run st_tgt), k_tgt (snd (run st_tgt))))
     :
-      _sim_itree sim_itree RR i_src0 i_tgt0 w0 (st_src0, i_src) (st_tgt0, trigger (SUpdate run) >>= k_tgt)
+      _sim_itree sim_itree RR f_src f_tgt w0 (st_src, i_src) (st_tgt, trigger (SUpdate run) >>= k_tgt)
 
   | sim_itree_progress
-      i_src0 i_tgt0 w0 (st_src0: st_local) (st_tgt0: st_local) i_src i_tgt
-      (SIM: sim_itree _ _ RR false false w0 (st_src0, i_src) (st_tgt0, i_tgt))
-      (SRC: i_src0 = true)
-      (TGT: i_tgt0 = true)
+      w0 st_src st_tgt 
+      i_src i_tgt
+      (SIM: sim_itree _ _ RR false false w0 (st_src, i_src) (st_tgt, i_tgt))
+
     :
-      _sim_itree sim_itree RR true true w0 (st_src0, i_src) (st_tgt0, i_tgt)
+      _sim_itree sim_itree RR true true w0 (st_src, i_src) (st_tgt, i_tgt)
   .
 
   Definition lift_rel {R_src R_tgt} (w0: world) (RR: R_src -> R_tgt -> Prop)
-             (st_src0: st_local) (st_tgt0: st_local) (ret_src ret_tgt: Any.t) :=
+             st_src st_tgt (ret_src ret_tgt: Any.t) :=
     exists w1 : world,
-      (<<WLE: le w0 w1 >> /\ <<WF: wf w1 (st_src0, st_tgt0) >> /\ <<RET: ret_src = ret_tgt >>).
-
-  Lemma _sim_itree_ind2 (sim_itree: forall (R_src R_tgt: Type) 
-                                    (RR: st_local -> st_local -> R_src -> R_tgt -> Prop), bool -> bool -> world -> st_local * itree Es R_src -> st_local * itree Es R_tgt -> Prop)
-        {R_src R_tgt} (RR: st_local -> st_local -> R_src -> R_tgt -> Prop)
-        (P: bool -> bool -> world -> st_local * itree Es R_src -> st_local * itree Es R_tgt -> Prop)
-        (RET: forall
-            i_src0 i_tgt0 w0 st_src0 st_tgt0
-            v_src v_tgt
-            (RET: RR st_src0 st_tgt0 v_src v_tgt),
-            P i_src0 i_tgt0 w0 (st_src0, Ret v_src) (st_tgt0, Ret v_tgt))
-        (CALL: forall
-            i_src0 i_tgt0 w w0 st_src0 st_tgt0
-            fn varg k_src k_tgt
-            (WF: wf w0 (st_src0, st_tgt0))
-            (K: forall w1 vret st_src1 st_tgt1 (WLE: le w0 w1) (WF: wf w1 (st_src1, st_tgt1)),
-                sim_itree _ _ RR true true w (st_src1, k_src vret) (st_tgt1, k_tgt vret)),
-            P i_src0 i_tgt0 w (st_src0, trigger (Call fn varg) >>= k_src)
-              (st_tgt0, trigger (Call fn varg) >>= k_tgt))
-        (SYSCALL: forall
-            i_src0 i_tgt0 w0 (st_src0: st_local) (st_tgt0: st_local)
-            fn varg rvs k_src k_tgt
-            (K: forall vret,
-                sim_itree _ _ RR true true w0 (st_src0, k_src vret) (st_tgt0, k_tgt vret)),
-            P i_src0 i_tgt0 w0 (st_src0, trigger (Syscall fn varg rvs) >>= k_src)
-              (st_tgt0, trigger (Syscall fn varg rvs) >>= k_tgt))
-        (INLINESRC: forall
-            i_src0 i_tgt0 w st_src st_tgt
-            f fn varg k_src i_tgt
-            (FUN: alist_find fn fl_src = Some f)
-            (* (IN: In (fn, f) fl_src )  *)
-            (K: _sim_itree sim_itree RR true i_tgt0 w (st_src, (f varg) >>= k_src) (st_tgt, i_tgt))
-            (IH: P true i_tgt0 w (st_src, (f varg) >>= k_src) (st_tgt, i_tgt)),
-            P i_src0 i_tgt0 w (st_src, trigger (Call fn varg) >>= k_src)
-              (st_tgt, i_tgt))
-        (INLINETGT: forall
-            i_src0 i_tgt0 w st_src st_tgt
-            f fn varg i_src k_tgt
-            (FUN: alist_find fn fl_tgt = Some f)
-            (* (IN: In (fn, f) fl_tgt )  *)
-            (K: _sim_itree sim_itree RR i_src0 true w (st_src, i_src) (st_tgt, (f varg) >>= k_tgt))
-            (IH: P i_src0 true w (st_src, i_src) (st_tgt, (f varg) >>= k_tgt)),
-            P i_src0 i_tgt0 w (st_src, i_src)
-              (st_tgt, trigger (Call fn varg) >>= k_tgt)) 
-        (TAUSRC: forall
-            i_src0 i_tgt0 w0 (st_src0: st_local) (st_tgt0: st_local)
-            i_src i_tgt
-            (K: _sim_itree sim_itree RR true i_tgt0 w0 (st_src0, i_src) (st_tgt0, i_tgt))
-            (IH: P true i_tgt0 w0 (st_src0, i_src) (st_tgt0, i_tgt)),
-            P i_src0 i_tgt0 w0 (st_src0, tau;; i_src) (st_tgt0, i_tgt))
-        (TAUTGT: forall
-            i_src0 i_tgt0 w0 (st_src0: st_local) (st_tgt0: st_local)
-            i_src i_tgt
-            (K: _sim_itree sim_itree RR i_src0 true w0 (st_src0, i_src) (st_tgt0, i_tgt))
-            (IH: P i_src0 true w0 (st_src0, i_src) (st_tgt0, i_tgt)),
-            P i_src0 i_tgt0 w0 (st_src0, i_src) (st_tgt0, tau;; i_tgt))
-        (CHOOSESRC: forall
-            i_src0 i_tgt0 w0 (st_src0: st_local) (st_tgt0: st_local)
-            X k_src i_tgt
-            (K: exists (x: X), <<SIM: _sim_itree sim_itree RR true i_tgt0 w0 (st_src0, k_src x) (st_tgt0, i_tgt)>> /\ <<IH: P true i_tgt0 w0 (st_src0, k_src x) (st_tgt0, i_tgt)>>),
-            P i_src0 i_tgt0 w0 (st_src0, trigger (Choose X) >>= k_src)
-              (st_tgt0, i_tgt))
-        (CHOOSETGT: forall
-            i_src0 i_tgt0 w0 (st_src0: st_local) (st_tgt0: st_local)
-            X i_src k_tgt
-            (K: forall (x: X), <<SIMH: _sim_itree sim_itree RR i_src0 true w0 (st_src0, i_src) (st_tgt0, k_tgt x)>> /\ <<IH: P i_src0 true w0 (st_src0, i_src) (st_tgt0, k_tgt x)>>),
-            P i_src0 i_tgt0 w0 (st_src0, i_src)
-              (st_tgt0, trigger (Choose X) >>= k_tgt))
-        (TAKESRC: forall
-            i_src0 i_tgt0 w0 (st_src0: st_local) (st_tgt0: st_local)
-            X k_src i_tgt
-            (K: forall (x: X), <<SIM: _sim_itree sim_itree RR true i_tgt0 w0 (st_src0, k_src x) (st_tgt0, i_tgt)>> /\ <<IH: P true i_tgt0 w0 (st_src0, k_src x) (st_tgt0, i_tgt)>>),
-            P i_src0 i_tgt0 w0 (st_src0, trigger (Take X) >>= k_src)
-              (st_tgt0, i_tgt))
-        (TAKETGT: forall
-            i_src0 i_tgt0 w0 (st_src0: st_local) (st_tgt0: st_local)
-            X i_src k_tgt
-            (K: exists (x: X), <<SIM:_sim_itree sim_itree RR i_src0 true w0 (st_src0, i_src) (st_tgt0, k_tgt x)>> /\ <<IH: P i_src0 true w0 (st_src0, i_src) (st_tgt0, k_tgt x)>>),
-            P i_src0 i_tgt0 w0 (st_src0, i_src)
-              (st_tgt0, trigger (Take X) >>= k_tgt))
-        (SUPDATESRC: forall
-            i_src0 i_tgt0 w0 (st_src0: st_local) (st_tgt0: st_local)
-            X k_src i_tgt
-            (run: st_local -> st_local * X )
-            (K: _sim_itree sim_itree RR true i_tgt0 w0 (fst (run st_src0), k_src (snd (run st_src0))) (st_tgt0, i_tgt))
-            (IH: P true i_tgt0 w0 (fst (run st_src0), k_src (snd (run st_src0))) (st_tgt0, i_tgt)),
-            P i_src0 i_tgt0 w0 (st_src0, trigger (SUpdate run) >>= k_src) (st_tgt0, i_tgt))
-        (SUPDATETGT: forall
-            i_src0 i_tgt0 w0 (st_src0: st_local) (st_tgt0: st_local)
-            X i_src k_tgt
-            (run: st_local -> st_local * X )
-            (K: _sim_itree sim_itree RR i_src0 true w0 (st_src0, i_src) (fst (run st_tgt0), k_tgt (snd (run st_tgt0))))
-            (IH: P i_src0 true w0 (st_src0, i_src) (fst (run st_tgt0), k_tgt (snd (run st_tgt0)))),
-            P i_src0 i_tgt0 w0 (st_src0, i_src) (st_tgt0, trigger (SUpdate run) >>= k_tgt))
-        (PROGRESS: forall
-            i_src0 i_tgt0 w0 (st_src0: st_local) (st_tgt0: st_local) i_src i_tgt
-            (SIM: sim_itree _ _ RR false false w0 (st_src0, i_src) (st_tgt0, i_tgt))
-            (SRC: i_src0 = true)
-            (TGT: i_tgt0 = true),
-            P true true w0 (st_src0, i_src) (st_tgt0, i_tgt))
-    :
-      forall i_src0 i_tgt0 w0 st_src st_tgt
-             (SIM: _sim_itree sim_itree RR i_src0 i_tgt0 w0 st_src st_tgt),
-        P i_src0 i_tgt0 w0 st_src st_tgt.
-  Proof.
-    fix IH 6. i. inv SIM.
-    { eapply RET; eauto. }
-    { eapply CALL; eauto. }
-    { eapply SYSCALL; eauto. }
-    { eapply INLINESRC; eauto. }
-    { eapply INLINETGT; eauto. }
-    { eapply TAUSRC; eauto. }
-    { eapply TAUTGT; eauto. }
-    { eapply CHOOSESRC; eauto. des. esplits; eauto. }
-    { eapply CHOOSETGT; eauto. }
-    { eapply TAKESRC; eauto. }
-    { eapply TAKETGT; eauto. des. esplits; eauto. }
-    { eapply SUPDATESRC; eauto. }
-    { eapply SUPDATETGT; eauto. }
-    { eapply PROGRESS; eauto. }
-
-  Qed.
+      (<<WLE: le w0 w1 >> /\ <<WF: wf w1 (st_src, st_tgt) >> /\ <<RET: ret_src = ret_tgt >>).
 
   Definition sim_itree o_src o_tgt w0 : relation _ :=
     paco8 _sim_itree bot8 _ _ (lift_rel w0 (@eq Any.t)) o_src o_tgt w0.
 
   Lemma sim_itree_mon: monotone8 _sim_itree.
   Proof.
-    ii. induction IN using _sim_itree_ind2; try (by des; econs; ss; et).
-    - econs; ss; et. ii. exploit K; et. i; des. esplits; et.
-    - econs; ss; et. ii. exploit K; et. i; des. esplits; et.
+    ii. induction IN; try (econs; et; ii; exploit K; i; des; et).
   Qed.
 
   Hint Constructors _sim_itree.
@@ -297,228 +172,212 @@ Section SIM.
         R_src R_tgt (RR: st_local -> st_local -> R_src -> R_tgt -> Prop) 
         (P: bool -> bool -> world -> st_local * itree Es R_src -> st_local * itree Es R_tgt -> Prop)
         (RET: forall
-            i_src0 i_tgt0 w0 st_src0 st_tgt0
+            f_src f_tgt w0 st_src st_tgt
             v_src v_tgt
-            (RET: RR st_src0 st_tgt0 v_src v_tgt),
-            P i_src0 i_tgt0 w0 (st_src0, Ret v_src) (st_tgt0, Ret v_tgt))
+            (RET: RR st_src st_tgt v_src v_tgt),
+            P f_src f_tgt w0 (st_src, Ret v_src) (st_tgt, Ret v_tgt))
         (CALL: forall
-            i_src0 i_tgt0 w w0 st_src0 st_tgt0
+            f_src f_tgt w w0 st_src st_tgt
             fn varg k_src k_tgt
-            (WF: wf w0 (st_src0, st_tgt0))
-            (K: forall w1 vret st_src1 st_tgt1 (WLE: le w0 w1) (WF: wf w1 (st_src1, st_tgt1)),
-                paco8 _sim_itree bot8 _ _ RR true true w (st_src1, k_src vret) (st_tgt1, k_tgt vret)),
-            P i_src0 i_tgt0 w (st_src0, trigger (Call fn varg) >>= k_src)
-              (st_tgt0, trigger (Call fn varg) >>= k_tgt))
+            (WF: wf w0 (st_src, st_tgt))
+            (K: forall w1 vret st_src0 st_tgt0 (WLE: le w0 w1) (WF: wf w1 (st_src0, st_tgt0)),
+                paco8 _sim_itree bot8 _ _ RR true true w (st_src0, k_src vret) (st_tgt0, k_tgt vret)),
+            P f_src f_tgt w (st_src, trigger (Call fn varg) >>= k_src)
+              (st_tgt, trigger (Call fn varg) >>= k_tgt))
         (SYSCALL: forall
-            i_src0 i_tgt0 w0 (st_src0: st_local) (st_tgt0: st_local)
+            f_src f_tgt w0 st_src st_tgt
             fn varg rvs k_src k_tgt
             (K: forall vret,
-                paco8 _sim_itree bot8 _ _ RR true true w0 (st_src0, k_src vret) (st_tgt0, k_tgt vret)),
-            P i_src0 i_tgt0 w0 (st_src0, trigger (Syscall fn varg rvs) >>= k_src)
-              (st_tgt0, trigger (Syscall fn varg rvs) >>= k_tgt))
+                paco8 _sim_itree bot8 _ _ RR true true w0 (st_src, k_src vret) (st_tgt, k_tgt vret)),
+            P f_src f_tgt w0 (st_src, trigger (Syscall fn varg rvs) >>= k_src)
+              (st_tgt, trigger (Syscall fn varg rvs) >>= k_tgt))
         (INLINESRC: forall
-            i_src0 i_tgt0 w0 st_src st_tgt
+            f_src f_tgt w0 st_src st_tgt
             f fn varg k_src i_tgt
             (FUN: alist_find fn fl_src = Some f)
-            (* (IN: In (fn, f) fl_src) *)
-            (K: paco8 _sim_itree bot8 _ _ RR true i_tgt0 w0 (st_src, (f varg) >>= k_src) (st_tgt, i_tgt))
-            (IH: P true i_tgt0 w0 (st_src, (f varg) >>= k_src) (st_tgt, i_tgt)),
-            P i_src0 i_tgt0 w0 (st_src, trigger (Call fn varg) >>= k_src) (st_tgt, i_tgt))
+            (K: paco8 _sim_itree bot8 _ _ RR true f_tgt w0 (st_src, (f varg) >>= k_src) (st_tgt, i_tgt))
+            (IH: P true f_tgt w0 (st_src, (f varg) >>= k_src) (st_tgt, i_tgt)),
+            P f_src f_tgt w0 (st_src, trigger (Call fn varg) >>= k_src) (st_tgt, i_tgt))
         (INLINETGT: forall
-            i_src0 i_tgt0 w0 st_src st_tgt
+            f_src f_tgt w0 st_src st_tgt
             f fn varg i_src k_tgt
             (FUN: alist_find fn fl_tgt = Some f)
-            (* (IN: In (fn, f) fl_tgt) *)
-            (K: paco8 _sim_itree bot8 _ _ RR i_src0 true w0 (st_src, i_src) (st_tgt, (f varg) >>= k_tgt))
-            (IH: P i_src0 true w0 (st_src, i_src) (st_tgt, (f varg) >>= k_tgt)),
-            P i_src0 i_tgt0 w0 (st_src, i_src) (st_tgt, trigger (Call fn varg) >>= k_tgt))            
+            (K: paco8 _sim_itree bot8 _ _ RR f_src true w0 (st_src, i_src) (st_tgt, (f varg) >>= k_tgt))
+            (IH: P f_src true w0 (st_src, i_src) (st_tgt, (f varg) >>= k_tgt)),
+            P f_src f_tgt w0 (st_src, i_src) (st_tgt, trigger (Call fn varg) >>= k_tgt))            
         (TAUSRC: forall
-            i_src0 i_tgt0 w0 (st_src0: st_local) (st_tgt0: st_local)
+            f_src f_tgt w0 st_src st_tgt
             i_src i_tgt
-            (K: paco8 _sim_itree bot8 _ _ RR true i_tgt0 w0 (st_src0, i_src) (st_tgt0, i_tgt))
-            (IH: P true i_tgt0 w0 (st_src0, i_src) (st_tgt0, i_tgt)),
-            P i_src0 i_tgt0 w0 (st_src0, tau;; i_src) (st_tgt0, i_tgt))
+            (K: paco8 _sim_itree bot8 _ _ RR true f_tgt w0 (st_src, i_src) (st_tgt, i_tgt))
+            (IH: P true f_tgt w0 (st_src, i_src) (st_tgt, i_tgt)),
+            P f_src f_tgt w0 (st_src, tau;; i_src) (st_tgt, i_tgt))
         (TAUTGT: forall
-            i_src0 i_tgt0 w0 (st_src0: st_local) (st_tgt0: st_local)
+            f_src f_tgt w0 st_src st_tgt
             i_src i_tgt
-            (K: paco8 _sim_itree bot8 _ _ RR i_src0 true w0 (st_src0, i_src) (st_tgt0, i_tgt))
-            (IH: P i_src0 true w0 (st_src0, i_src) (st_tgt0, i_tgt)),
-            P i_src0 i_tgt0 w0 (st_src0, i_src) (st_tgt0, tau;; i_tgt))            
+            (K: paco8 _sim_itree bot8 _ _ RR f_src true w0 (st_src, i_src) (st_tgt, i_tgt))
+            (IH: P f_src true w0 (st_src, i_src) (st_tgt, i_tgt)),
+            P f_src f_tgt w0 (st_src, i_src) (st_tgt, tau;; i_tgt))            
         (CHOOSESRC: forall
-            i_src0 i_tgt0 w0 (st_src0: st_local) (st_tgt0: st_local)
-            X k_src i_tgt
-            (K: exists (x: X), <<SIM: paco8 _sim_itree bot8 _ _ RR true i_tgt0 w0 (st_src0, k_src x) (st_tgt0, i_tgt)>> /\ <<IH: P true i_tgt0 w0 (st_src0, k_src x) (st_tgt0, i_tgt)>>),
-            P i_src0 i_tgt0 w0 (st_src0, trigger (Choose X) >>= k_src)
-              (st_tgt0, i_tgt))
+            f_src f_tgt w0 st_src st_tgt
+            X x k_src i_tgt
+            (K: paco8 _sim_itree bot8 _ _ RR true f_tgt w0 (st_src, k_src x) (st_tgt, i_tgt))
+            (IH: P true f_tgt w0 (st_src, k_src x) (st_tgt, i_tgt)),
+            P f_src f_tgt w0 (st_src, trigger (Choose X) >>= k_src)
+              (st_tgt, i_tgt))
         (CHOOSETGT: forall
-            i_src0 i_tgt0 w0 (st_src0: st_local) (st_tgt0: st_local)
+            f_src f_tgt w0 st_src st_tgt
             X i_src k_tgt
-            (K: forall (x: X), <<SIMH: paco8 _sim_itree bot8 _ _ RR i_src0 true w0 (st_src0, i_src) (st_tgt0, k_tgt x)>> /\ <<IH: P i_src0 true w0 (st_src0, i_src) (st_tgt0, k_tgt x)>>),
-            P i_src0 i_tgt0 w0 (st_src0, i_src)
-              (st_tgt0, trigger (Choose X) >>= k_tgt))
+            (K: forall (x: X), <<SIMH: paco8 _sim_itree bot8 _ _ RR f_src true w0 (st_src, i_src) (st_tgt, k_tgt x)>> /\ <<IH: P f_src true w0 (st_src, i_src) (st_tgt, k_tgt x)>>),
+            P f_src f_tgt w0 (st_src, i_src)
+              (st_tgt, trigger (Choose X) >>= k_tgt))
         (TAKESRC: forall
-            i_src0 i_tgt0 w0 (st_src0: st_local) (st_tgt0: st_local)
+            f_src f_tgt w0 st_src st_tgt
             X k_src i_tgt
-            (K: forall (x: X), <<SIM: paco8 _sim_itree bot8 _ _ RR true i_tgt0 w0 (st_src0, k_src x) (st_tgt0, i_tgt)>> /\ <<IH: P true i_tgt0 w0 (st_src0, k_src x) (st_tgt0, i_tgt)>>),
-            P i_src0 i_tgt0 w0 (st_src0, trigger (Take X) >>= k_src)
-              (st_tgt0, i_tgt))
+            (K: forall (x: X), <<SIM: paco8 _sim_itree bot8 _ _ RR true f_tgt w0 (st_src, k_src x) (st_tgt, i_tgt)>> /\ <<IH: P true f_tgt w0 (st_src, k_src x) (st_tgt, i_tgt)>>),
+            P f_src f_tgt w0 (st_src, trigger (Take X) >>= k_src)
+              (st_tgt, i_tgt))
         (TAKETGT: forall
-            i_src0 i_tgt0 w0 (st_src0: st_local) (st_tgt0: st_local)
-            X i_src k_tgt
-            (K: exists (x: X), <<SIM:paco8 _sim_itree bot8 _ _ RR i_src0 true w0 (st_src0, i_src) (st_tgt0, k_tgt x)>> /\ <<IH: P i_src0 true w0 (st_src0, i_src) (st_tgt0, k_tgt x)>>),
-            P i_src0 i_tgt0 w0 (st_src0, i_src)
-              (st_tgt0, trigger (Take X) >>= k_tgt))
+            f_src f_tgt w0 st_src st_tgt
+            X x i_src k_tgt
+            (K: paco8 _sim_itree bot8 _ _ RR f_src true w0 (st_src, i_src) (st_tgt, k_tgt x))
+            (IH: P f_src true w0 (st_src, i_src) (st_tgt, k_tgt x)),
+            P f_src f_tgt w0 (st_src, i_src)
+              (st_tgt, trigger (Take X) >>= k_tgt))
         (SUPDATESRC: forall
-            i_src0 i_tgt0 w0 (st_src0: st_local) (st_tgt0: st_local)
+            f_src f_tgt w0 st_src st_tgt
             X k_src i_tgt
             (run: st_local -> st_local * X )
-            (K: paco8 _sim_itree bot8 _ _ RR true i_tgt0 w0 (fst (run st_src0), k_src (snd (run st_src0))) (st_tgt0, i_tgt))
-            (IH: P true i_tgt0 w0 (fst (run st_src0), k_src (snd (run st_src0))) (st_tgt0, i_tgt)),
-            P i_src0 i_tgt0 w0 (st_src0, trigger (SUpdate run) >>= k_src) (st_tgt0, i_tgt))
+            (K: paco8 _sim_itree bot8 _ _ RR true f_tgt w0 (fst (run st_src), k_src (snd (run st_src))) (st_tgt, i_tgt))
+            (IH: P true f_tgt w0 (fst (run st_src), k_src (snd (run st_src))) (st_tgt, i_tgt)),
+            P f_src f_tgt w0 (st_src, trigger (SUpdate run) >>= k_src) (st_tgt, i_tgt))
         (SUPDATETGT: forall
-            i_src0 i_tgt0 w0 (st_src0: st_local) (st_tgt0: st_local)
+            f_src f_tgt w0 st_src st_tgt
             X i_src k_tgt
             (run: st_local -> st_local * X )
-            (K: paco8 _sim_itree bot8 _ _ RR i_src0 true w0 (st_src0, i_src) (fst (run st_tgt0), k_tgt (snd (run st_tgt0))))
-            (IH:  P i_src0 true w0 (st_src0, i_src) (fst (run st_tgt0), k_tgt (snd (run st_tgt0)))),
+            (K: paco8 _sim_itree bot8 _ _ RR f_src true w0 (st_src, i_src) (fst (run st_tgt), k_tgt (snd (run st_tgt))))
+            (IH:  P f_src true w0 (st_src, i_src) (fst (run st_tgt), k_tgt (snd (run st_tgt)))),
 
-            P i_src0 i_tgt0 w0 (st_src0, i_src) (st_tgt0, trigger (SUpdate run) >>= k_tgt))       
+            P f_src f_tgt w0 (st_src, i_src) (st_tgt, trigger (SUpdate run) >>= k_tgt))       
         (PROGRESS: forall
-            i_src0 i_tgt0 w0 (st_src0: st_local) (st_tgt0: st_local)
+            w0 st_src st_tgt
             i_src i_tgt
-            (SIM: paco8 _sim_itree bot8 _ _ RR false false w0 (st_src0, i_src) (st_tgt0, i_tgt))
-            (SRC: i_src0 = true)
-            (TGT: i_tgt0 = true),
-            P true true w0 (st_src0, i_src) (st_tgt0, i_tgt))
+            (SIM: paco8 _sim_itree bot8 _ _ RR false false w0 (st_src, i_src) (st_tgt, i_tgt)),
+            P true true w0 (st_src, i_src) (st_tgt, i_tgt))
     :
-      forall i_src0 i_tgt0 w0 st_src st_tgt
-             (SIM: paco8 _sim_itree bot8 _ _ RR i_src0 i_tgt0 w0 st_src st_tgt),
-        P i_src0 i_tgt0 w0 st_src st_tgt.
+      forall f_src f_tgt w0 st_src st_tgt
+             (SIM: paco8 _sim_itree bot8 _ _ RR f_src f_tgt w0 st_src st_tgt),
+        P f_src f_tgt w0 st_src st_tgt.
   Proof.
-    i. punfold SIM. induction SIM using _sim_itree_ind2.
-    { eapply RET; eauto. }
-    { eapply CALL; eauto. i. exploit K; eauto. i. pclearbot. eauto. }
-    { eapply SYSCALL; eauto. i. exploit K; eauto. i. pclearbot. eauto. }
-    { eapply INLINESRC; et. }
-    { eapply INLINETGT; et. }
-    { eapply TAUSRC; eauto. }
-    { eapply TAUTGT; eauto. }
-    { eapply CHOOSESRC; eauto. des. esplits; eauto. }
-    { eapply CHOOSETGT; eauto. i. exploit K; eauto. i. des.
-    pclearbot. esplits; eauto. }
-    { eapply TAKESRC; eauto. i. exploit K; eauto. i. des.
-      pclearbot. esplits; eauto. }
-    { eapply TAKETGT; eauto. des. esplits; eauto. }
-    { eapply SUPDATESRC; eauto. }
-    { eapply SUPDATETGT; eauto. }
+    i. punfold SIM. induction SIM; et.
+    { eapply CHOOSETGT; eauto. }
+    { eapply TAKESRC; eauto. }
     { eapply PROGRESS; eauto. pclearbot. auto. }
-
   Qed.
 
   Variant sim_itree_indC (sim_itree: forall (R_src R_tgt: Type) (RR: st_local -> st_local -> R_src -> R_tgt -> Prop), bool -> bool -> world -> st_local * itree Es R_src -> st_local * itree Es R_tgt -> Prop)
           {R_src R_tgt} (RR: st_local -> st_local -> R_src -> R_tgt -> Prop)
     : bool -> bool -> world -> st_local * itree Es R_src -> st_local * itree Es R_tgt -> Prop :=
   | sim_itree_indC_ret
-      i_src0 i_tgt0 w0 st_src0 st_tgt0
+      f_src f_tgt w0 st_src st_tgt
       v_src v_tgt
-      (RET: RR st_src0 st_tgt0 v_src v_tgt)
+      (RET: RR st_src st_tgt v_src v_tgt)
     :
-      sim_itree_indC  sim_itree RR i_src0 i_tgt0 w0 (st_src0, Ret v_src) (st_tgt0, Ret v_tgt)
+      sim_itree_indC  sim_itree RR f_src f_tgt w0 (st_src, Ret v_src) (st_tgt, Ret v_tgt)
   | sim_itree_indC_call
-      i_src0 i_tgt0 w w0 st_src0 st_tgt0
+      f_src f_tgt w w0 st_src st_tgt
       fn varg k_src k_tgt
-      (WF: wf w0 (st_src0, st_tgt0))
-      (K: forall w1 vret st_src1 st_tgt1 (WLE: le w0 w1) (WF: wf w1 (st_src1, st_tgt1)),
-          sim_itree _ _ RR true true w (st_src1, k_src vret) (st_tgt1, k_tgt vret))
+      (WF: wf w0 (st_src, st_tgt))
+      (K: forall w1 vret st_src0 st_tgt0 (WLE: le w0 w1) (WF: wf w1 (st_src0, st_tgt0)),
+          sim_itree _ _ RR true true w (st_src0, k_src vret) (st_tgt0, k_tgt vret))
     :
-      sim_itree_indC  sim_itree RR i_src0 i_tgt0 w (st_src0, trigger (Call fn varg) >>= k_src)
-                     (st_tgt0, trigger (Call fn varg) >>= k_tgt)
+      sim_itree_indC  sim_itree RR f_src f_tgt w (st_src, trigger (Call fn varg) >>= k_src)
+                     (st_tgt, trigger (Call fn varg) >>= k_tgt)
   | sim_itree_indC_syscall
-      i_src0 i_tgt0 w0 (st_src0: st_local) (st_tgt0: st_local)
+      f_src f_tgt w0 st_src st_tgt
       fn varg rvs k_src k_tgt
       (K: forall vret,
-          sim_itree _ _ RR true true w0 (st_src0, k_src vret) (st_tgt0, k_tgt vret))
+          sim_itree _ _ RR true true w0 (st_src, k_src vret) (st_tgt, k_tgt vret))
     :
-      sim_itree_indC  sim_itree RR i_src0 i_tgt0 w0 (st_src0, trigger (Syscall fn varg rvs) >>= k_src)
-                     (st_tgt0, trigger (Syscall fn varg rvs) >>= k_tgt)
+      sim_itree_indC  sim_itree RR f_src f_tgt w0 (st_src, trigger (Syscall fn varg rvs) >>= k_src)
+                     (st_tgt, trigger (Syscall fn varg rvs) >>= k_tgt)
 
   | sim_itree_indC_inline_src
-      i_src0 i_tgt0 w0 (st_src0: st_local) (st_tgt0: st_local)
+      f_src f_tgt w0 st_src st_tgt
       f fn varg k_src i_tgt
       (FUN: alist_find fn fl_src = Some f)
       (* (IN: In (fn, f) fl_src) *)
-      (K: sim_itree _ _ RR true i_tgt0 w0 (st_src0, (f varg) >>= k_src) (st_tgt0, i_tgt))
+      (K: sim_itree _ _ RR true f_tgt w0 (st_src, (f varg) >>= k_src) (st_tgt, i_tgt))
     :
-      sim_itree_indC  sim_itree RR i_src0 i_tgt0 w0 (st_src0, trigger (Call fn varg) >>= k_src) (st_tgt0, i_tgt)
+      sim_itree_indC  sim_itree RR f_src f_tgt w0 (st_src, trigger (Call fn varg) >>= k_src) (st_tgt, i_tgt)
 
   | sim_itree_indC_inline_tgt
-      i_src0 i_tgt0 w0 (st_src0: st_local) (st_tgt0: st_local)
+      f_src f_tgt w0 st_src st_tgt
       f fn varg i_src k_tgt
       (FUN: alist_find fn fl_tgt = Some f)
       (* (IN: In (fn, f) fl_tgt) *)
-      (K: sim_itree _ _ RR i_src0 true w0 (st_src0, i_src) (st_tgt0, (f varg) >>= k_tgt))
+      (K: sim_itree _ _ RR f_src true w0 (st_src, i_src) (st_tgt, (f varg) >>= k_tgt))
     :
-      sim_itree_indC  sim_itree RR i_src0 i_tgt0 w0 (st_src0, i_src) (st_tgt0, trigger (Call fn varg) >>= k_tgt)
+      sim_itree_indC  sim_itree RR f_src f_tgt w0 (st_src, i_src) (st_tgt, trigger (Call fn varg) >>= k_tgt)
  
   | sim_itree_indC_tau_src
-      i_src0 i_tgt0 w0 (st_src0: st_local) (st_tgt0: st_local)
+      f_src f_tgt w0 st_src st_tgt
       i_src i_tgt
-      (K: sim_itree _ _ RR true i_tgt0 w0 (st_src0, i_src) (st_tgt0, i_tgt))
+      (K: sim_itree _ _ RR true f_tgt w0 (st_src, i_src) (st_tgt, i_tgt))
     :
-      sim_itree_indC  sim_itree RR i_src0 i_tgt0 w0 (st_src0, tau;; i_src) (st_tgt0, i_tgt)
+      sim_itree_indC  sim_itree RR f_src f_tgt w0 (st_src, tau;; i_src) (st_tgt, i_tgt)
 
   | sim_itree_indC_tau_tgt
-      i_src0 i_tgt0 w0 (st_src0: st_local) (st_tgt0: st_local)
+      f_src f_tgt w0 st_src st_tgt
       i_src i_tgt
-      (K: sim_itree _ _ RR i_src0 true w0 (st_src0, i_src) (st_tgt0, i_tgt))
+      (K: sim_itree _ _ RR f_src true w0 (st_src, i_src) (st_tgt, i_tgt))
     :
-      sim_itree_indC  sim_itree RR i_src0 i_tgt0 w0 (st_src0, i_src) (st_tgt0, tau;; i_tgt)
+      sim_itree_indC  sim_itree RR f_src f_tgt w0 (st_src, i_src) (st_tgt, tau;; i_tgt)
 
   | sim_itree_indC_choose_src
-      i_src0 i_tgt0 w0 (st_src0: st_local) (st_tgt0: st_local)
-      X k_src i_tgt
-      (K: exists (x: X), sim_itree _ _ RR true i_tgt0 w0 (st_src0, k_src x) (st_tgt0, i_tgt))
+      f_src f_tgt w0 st_src st_tgt
+      X x k_src i_tgt
+      (K: sim_itree _ _ RR true f_tgt w0 (st_src, k_src x) (st_tgt, i_tgt))
     :
-      sim_itree_indC  sim_itree RR i_src0 i_tgt0 w0 (st_src0, trigger (Choose X) >>= k_src)
-                     (st_tgt0, i_tgt)
+      sim_itree_indC  sim_itree RR f_src f_tgt w0 (st_src, trigger (Choose X) >>= k_src)
+                     (st_tgt, i_tgt)
   | sim_itree_indC_choose_tgt
-      i_src0 i_tgt0 w0 (st_src0: st_local) (st_tgt0: st_local)
+      f_src f_tgt w0 st_src st_tgt
       X i_src k_tgt
-      (K: forall (x: X), sim_itree _ _ RR i_src0 true w0 (st_src0, i_src) (st_tgt0, k_tgt x))
+      (K: forall (x: X), sim_itree _ _ RR f_src true w0 (st_src, i_src) (st_tgt, k_tgt x))
     :
-      sim_itree_indC  sim_itree RR i_src0 i_tgt0 w0 (st_src0, i_src)
-                     (st_tgt0, trigger (Choose X) >>= k_tgt)
+      sim_itree_indC  sim_itree RR f_src f_tgt w0 (st_src, i_src)
+                     (st_tgt, trigger (Choose X) >>= k_tgt)
 
   | sim_itree_indC_take_src
-      i_src0 i_tgt0 w0 (st_src0: st_local) (st_tgt0: st_local)
+      f_src f_tgt w0 st_src st_tgt
       X k_src i_tgt
-      (K: forall (x: X), sim_itree _ _ RR true i_tgt0 w0 (st_src0, k_src x) (st_tgt0, i_tgt))
+      (K: forall (x: X), sim_itree _ _ RR true f_tgt w0 (st_src, k_src x) (st_tgt, i_tgt))
     :
-      sim_itree_indC  sim_itree RR i_src0 i_tgt0 w0 (st_src0, trigger (Take X) >>= k_src)
-                     (st_tgt0, i_tgt)
+      sim_itree_indC  sim_itree RR f_src f_tgt w0 (st_src, trigger (Take X) >>= k_src)
+                     (st_tgt, i_tgt)
   | sim_itree_indC_take_tgt
-      i_src0 i_tgt0 w0 (st_src0: st_local) (st_tgt0: st_local)
-      X i_src k_tgt
-      (K: exists (x: X), sim_itree _ _ RR i_src0 true w0 (st_src0, i_src) (st_tgt0, k_tgt x))
+      f_src f_tgt w0 st_src st_tgt
+      X x i_src k_tgt
+      (K: sim_itree _ _ RR f_src true w0 (st_src, i_src) (st_tgt, k_tgt x))
     :
-      sim_itree_indC  sim_itree RR i_src0 i_tgt0 w0 (st_src0, i_src)
-                     (st_tgt0, trigger (Take X) >>= k_tgt)
+      sim_itree_indC  sim_itree RR f_src f_tgt w0 (st_src, i_src)
+                     (st_tgt, trigger (Take X) >>= k_tgt)
   
   | sim_itree_indC_supdate_src
-      i_src0 i_tgt0 w0 (st_src0: st_local) (st_tgt0: st_local)
+      f_src f_tgt w0 st_src st_tgt
       X k_src i_tgt
       (run: st_local -> st_local * X )
-      (K: sim_itree _ _ RR true i_tgt0 w0 (fst (run st_src0), k_src (snd (run st_src0))) (st_tgt0, i_tgt))
+      (K: sim_itree _ _ RR true f_tgt w0 (fst (run st_src), k_src (snd (run st_src))) (st_tgt, i_tgt))
     :
-      sim_itree_indC  sim_itree RR i_src0 i_tgt0 w0 (st_src0, trigger (SUpdate run) >>= k_src) (st_tgt0, i_tgt)
+      sim_itree_indC  sim_itree RR f_src f_tgt w0 (st_src, trigger (SUpdate run) >>= k_src) (st_tgt, i_tgt)
 
   | sim_itree_indC_supdate_tgt
-      i_src0 i_tgt0 w0 (st_src0: st_local) (st_tgt0: st_local)
+      f_src f_tgt w0 st_src st_tgt
       X i_src k_tgt
       (run: st_local -> st_local * X )
-      (K: sim_itree _ _ RR i_src0 true w0 (st_src0, i_src) (fst (run st_tgt0), k_tgt (snd (run st_tgt0))))
+      (K: sim_itree _ _ RR f_src true w0 (st_src, i_src) (fst (run st_tgt), k_tgt (snd (run st_tgt))))
     :
-      sim_itree_indC  sim_itree RR i_src0 i_tgt0 w0 (st_src0, i_src) (st_tgt0, trigger (SUpdate run) >>= k_tgt)
+      sim_itree_indC  sim_itree RR f_src f_tgt w0 (st_src, i_src) (st_tgt, trigger (SUpdate run) >>= k_tgt)
   .
 
   Lemma sim_itree_indC_mon: monotone8 sim_itree_indC.
@@ -533,9 +392,8 @@ Section SIM.
     eapply wrespect8_uclo; eauto with paco.
     econs; eauto with paco. i. inv PR.
     { econs 1; eauto. }
-    { econs 2; eauto. i. exploit K; eauto. i. des.
-      esplits; eauto. eapply rclo8_base. eauto. }
-    { econs 3; eauto. i. eapply rclo8_base. eauto. }
+    { econs 2; eauto. i. eapply sim_itree_mon; et. i. eapply rclo8_base. et. }
+    { econs 3; eauto. i. eapply sim_itree_mon; et. i. eapply rclo8_base. eauto. }
     { econs 4; et. eapply sim_itree_mon; et. eapply rclo8_base. }
     { econs 5; et. eapply sim_itree_mon; et. eapply rclo8_base. }
     { econs 6; eauto. eapply sim_itree_mon; eauto. i. eapply rclo8_base. eauto. }
@@ -552,105 +410,105 @@ Section SIM.
           {R_src R_tgt} (RR: st_local -> st_local -> R_src -> R_tgt -> Prop)
     : bool -> bool -> world -> st_local * itree Es R_src -> st_local * itree Es R_tgt -> Prop :=
   | sim_itreeC_ret
-      i_src0 i_tgt0 w0 st_src0 st_tgt0
+      f_src f_tgt w0 st_src st_tgt
       v_src v_tgt
-      (RET: RR st_src0 st_tgt0 v_src v_tgt)
+      (RET: RR st_src st_tgt v_src v_tgt)
     :
-      sim_itreeC r g RR i_src0 i_tgt0 w0 (st_src0, Ret v_src) (st_tgt0, Ret v_tgt)
+      sim_itreeC r g RR f_src f_tgt w0 (st_src, Ret v_src) (st_tgt, Ret v_tgt)
   | sim_itreeC_call
-      i_src0 i_tgt0 w w0 st_src0 st_tgt0
+      f_src f_tgt w w0 st_src st_tgt
       fn varg k_src k_tgt
-      (WF: wf w0 (st_src0, st_tgt0))
-      (K: forall w1 vret st_src1 st_tgt1 (WLE: le w0 w1) (WF: wf w1 (st_src1, st_tgt1)),
-          g _ _ RR true true w (st_src1, k_src vret) (st_tgt1, k_tgt vret))
+      (WF: wf w0 (st_src, st_tgt))
+      (K: forall w1 vret st_src0 st_tgt0 (WLE: le w0 w1) (WF: wf w1 (st_src0, st_tgt0)),
+          r _ _ RR true true w (st_src0, k_src vret) (st_tgt0, k_tgt vret))
     :
-      sim_itreeC r g RR i_src0 i_tgt0 w (st_src0, trigger (Call fn varg) >>= k_src)
-                 (st_tgt0, trigger (Call fn varg) >>= k_tgt)
+      sim_itreeC r g RR f_src f_tgt w (st_src, trigger (Call fn varg) >>= k_src)
+                 (st_tgt, trigger (Call fn varg) >>= k_tgt)
   | sim_itreeC_syscall
-      i_src0 i_tgt0 w0 (st_src0: st_local) (st_tgt0: st_local)
+      f_src f_tgt w0 st_src st_tgt
       fn varg rvs k_src k_tgt
       (K: forall vret,
-          g _ _ RR true true w0 (st_src0, k_src vret) (st_tgt0, k_tgt vret))
+          r _ _ RR true true w0 (st_src, k_src vret) (st_tgt, k_tgt vret))
     :
-      sim_itreeC r g RR i_src0 i_tgt0 w0 (st_src0, trigger (Syscall fn varg rvs) >>= k_src)
-                 (st_tgt0, trigger (Syscall fn varg rvs) >>= k_tgt)
+      sim_itreeC r g RR f_src f_tgt w0 (st_src, trigger (Syscall fn varg rvs) >>= k_src)
+                 (st_tgt, trigger (Syscall fn varg rvs) >>= k_tgt)
 
   | sim_itreeC_inline_src
-      i_src0 i_tgt0 w0 (st_src0: st_local) (st_tgt0: st_local)
+      f_src f_tgt w0 st_src st_tgt
       f fn varg k_src i_tgt
       (FUN: alist_find fn fl_src = Some f)
       (* (IN: In (fn, f) fl_src) *)
-      (K: r _ _ RR true i_tgt0 w0 (st_src0, (f varg) >>= k_src) (st_tgt0, i_tgt))
+      (K: r _ _ RR true f_tgt w0 (st_src, (f varg) >>= k_src) (st_tgt, i_tgt))
     :
-      sim_itreeC r g RR i_src0 i_tgt0 w0 (st_src0, trigger (Call fn varg) >>= k_src) (st_tgt0, i_tgt)
+      sim_itreeC r g RR f_src f_tgt w0 (st_src, trigger (Call fn varg) >>= k_src) (st_tgt, i_tgt)
 
   | sim_itreeC_inline_tgt
-      i_src0 i_tgt0 w0 (st_src0: st_local) (st_tgt0: st_local)
+      f_src f_tgt w0 st_src st_tgt
       f fn varg i_src k_tgt
       (FUN: alist_find fn fl_tgt = Some f)
       (* (IN: In (fn, f) fl_tgt) *)
-      (K: r _ _ RR i_src0 true w0 (st_src0, i_src) (st_tgt0, (f varg) >>= k_tgt))
+      (K: r _ _ RR f_src true w0 (st_src, i_src) (st_tgt, (f varg) >>= k_tgt))
     :
-      sim_itreeC r g RR i_src0 i_tgt0 w0 (st_src0, i_src) (st_tgt0, trigger (Call fn varg) >>= k_tgt)
+      sim_itreeC r g RR f_src f_tgt w0 (st_src, i_src) (st_tgt, trigger (Call fn varg) >>= k_tgt)
 
   | sim_itreeC_tau_src
-      i_src0 i_tgt0 w0 (st_src0: st_local) (st_tgt0: st_local)
+      f_src f_tgt w0 st_src st_tgt
       i_src i_tgt
-      (K: r _ _ RR true i_tgt0 w0 (st_src0, i_src) (st_tgt0, i_tgt))
+      (K: r _ _ RR true f_tgt w0 (st_src, i_src) (st_tgt, i_tgt))
     :
-      sim_itreeC r g RR i_src0 i_tgt0 w0 (st_src0, tau;; i_src) (st_tgt0, i_tgt)
+      sim_itreeC r g RR f_src f_tgt w0 (st_src, tau;; i_src) (st_tgt, i_tgt)
 
   | sim_itreeC_tau_tgt
-      i_src0 i_tgt0 w0 (st_src0: st_local) (st_tgt0: st_local)
+      f_src f_tgt w0 st_src st_tgt
       i_src i_tgt
-      (K: r _ _ RR i_src0 true w0 (st_src0, i_src) (st_tgt0, i_tgt))
+      (K: r _ _ RR f_src true w0 (st_src, i_src) (st_tgt, i_tgt))
     :
-      sim_itreeC r g RR i_src0 i_tgt0 w0 (st_src0, i_src) (st_tgt0, tau;; i_tgt)
+      sim_itreeC r g RR f_src f_tgt w0 (st_src, i_src) (st_tgt, tau;; i_tgt)
 
 
   | sim_itreeC_choose_src
-      i_src0 i_tgt0 w0 (st_src0: st_local) (st_tgt0: st_local)
-      X k_src i_tgt
-      (K: exists (x: X), r _ _ RR true i_tgt0 w0 (st_src0, k_src x) (st_tgt0, i_tgt))
+      f_src f_tgt w0 st_src st_tgt
+      X x k_src i_tgt
+      (K: r _ _ RR true f_tgt w0 (st_src, k_src x) (st_tgt, i_tgt))
     :
-      sim_itreeC r g RR i_src0 i_tgt0 w0 (st_src0, trigger (Choose X) >>= k_src)
-                 (st_tgt0, i_tgt)
+      sim_itreeC r g RR f_src f_tgt w0 (st_src, trigger (Choose X) >>= k_src)
+                 (st_tgt, i_tgt)
   | sim_itreeC_choose_tgt
-      i_src0 i_tgt0 w0 (st_src0: st_local) (st_tgt0: st_local)
+      f_src f_tgt w0 st_src st_tgt
       X i_src k_tgt
-      (K: forall (x: X), r _ _ RR i_src0 true w0 (st_src0, i_src) (st_tgt0, k_tgt x))
+      (K: forall (x: X), r _ _ RR f_src true w0 (st_src, i_src) (st_tgt, k_tgt x))
     :
-      sim_itreeC r g RR i_src0 i_tgt0 w0 (st_src0, i_src)
-                 (st_tgt0, trigger (Choose X) >>= k_tgt)
+      sim_itreeC r g RR f_src f_tgt w0 (st_src, i_src)
+                 (st_tgt, trigger (Choose X) >>= k_tgt)
   | sim_itreeC_take_src
-      i_src0 i_tgt0 w0 (st_src0: st_local) (st_tgt0: st_local)
+      f_src f_tgt w0 st_src st_tgt
       X k_src i_tgt
-      (K: forall (x: X), r _ _ RR true i_tgt0 w0 (st_src0, k_src x) (st_tgt0, i_tgt))
+      (K: forall (x: X), r _ _ RR true f_tgt w0 (st_src, k_src x) (st_tgt, i_tgt))
     :
-      sim_itreeC r g RR i_src0 i_tgt0 w0 (st_src0, trigger (Take X) >>= k_src)
-                 (st_tgt0, i_tgt)
+      sim_itreeC r g RR f_src f_tgt w0 (st_src, trigger (Take X) >>= k_src)
+                 (st_tgt, i_tgt)
   | sim_itreeC_take_tgt
-      i_src0 i_tgt0 w0 (st_src0: st_local) (st_tgt0: st_local)
-      X i_src k_tgt
-      (K: exists (x: X), r _ _ RR i_src0 true w0 (st_src0, i_src) (st_tgt0, k_tgt x))
+      f_src f_tgt w0 st_src st_tgt
+      X x i_src k_tgt
+      (K: r _ _ RR f_src true w0 (st_src, i_src) (st_tgt, k_tgt x))
     :
-      sim_itreeC r g RR i_src0 i_tgt0 w0 (st_src0, i_src)
-                 (st_tgt0, trigger (Take X) >>= k_tgt)
+      sim_itreeC r g RR f_src f_tgt w0 (st_src, i_src)
+                 (st_tgt, trigger (Take X) >>= k_tgt)
   | sim_itreeC_supdate_src
-      i_src0 i_tgt0 w0 (st_src0: st_local) (st_tgt0: st_local)
+      f_src f_tgt w0 st_src st_tgt
       X k_src i_tgt
       (run: st_local -> st_local * X )
-      (K: r _ _ RR true i_tgt0 w0 (fst (run st_src0), k_src (snd (run st_src0))) (st_tgt0, i_tgt))
+      (K: r _ _ RR true f_tgt w0 (fst (run st_src), k_src (snd (run st_src))) (st_tgt, i_tgt))
     :
-      sim_itreeC r g RR i_src0 i_tgt0 w0 (st_src0, trigger (SUpdate run) >>= k_src) (st_tgt0, i_tgt)
+      sim_itreeC r g RR f_src f_tgt w0 (st_src, trigger (SUpdate run) >>= k_src) (st_tgt, i_tgt)
 
   | sim_itreeC_supdate_tgt
-      i_src0 i_tgt0 w0 (st_src0: st_local) (st_tgt0: st_local)
+      f_src f_tgt w0 st_src st_tgt
       X i_src k_tgt
       (run: st_local -> st_local * X )
-      (K: r _ _ RR i_src0 true w0 (st_src0, i_src) (fst (run st_tgt0), k_tgt (snd (run st_tgt0))))
+      (K: r _ _ RR f_src true w0 (st_src, i_src) (fst (run st_tgt), k_tgt (snd (run st_tgt))))
     :
-      sim_itreeC r g RR i_src0 i_tgt0 w0 (st_src0, i_src) (st_tgt0, trigger (SUpdate run) >>= k_tgt)
+      sim_itreeC r g RR f_src f_tgt w0 (st_src, i_src) (st_tgt, trigger (SUpdate run) >>= k_tgt)
 
   .
 
@@ -659,8 +517,8 @@ Section SIM.
   Proof.
     i. inv PR.
     { gstep. econs 1; eauto. }
-    { gstep. econs 2; eauto. i. gbase. eauto. }
-    { gstep. econs 3; eauto. i. gbase. eauto. }
+    { guclo sim_itree_indC_spec. econs 2; et. i. gbase. et. }
+    { guclo sim_itree_indC_spec. econs 3; et. i. gbase. et. }
     { guclo sim_itree_indC_spec. econs 4; eauto. gbase. eauto. }
     { guclo sim_itree_indC_spec. econs 5; eauto. gbase. eauto. }
     { guclo sim_itree_indC_spec. econs 6; eauto. gbase. eauto. }
@@ -686,12 +544,12 @@ Section SIM.
     { i. eapply gupaco8_mon; eauto. }
   Qed.
 
-  Lemma sim_itree_progress_flag R0 R1 RR w r g st_src0 st_tgt0
-        (SIM: gpaco8 _sim_itree (cpn8 _sim_itree) g g R0 R1 RR false false w st_src0 st_tgt0)
+  Lemma sim_itree_progress_flag R0 R1 RR w r g st_src st_tgt
+        (SIM: gpaco8 _sim_itree (cpn8 _sim_itree) g g R0 R1 RR false false w st_src st_tgt)
     :
-      gpaco8 _sim_itree (cpn8 _sim_itree) r g R0 R1 RR true true w st_src0 st_tgt0.
+      gpaco8 _sim_itree (cpn8 _sim_itree) r g R0 R1 RR true true w st_src st_tgt.
   Proof.
-    gstep. destruct st_src0, st_tgt0. econs; eauto. 
+    gstep. destruct st_src, st_tgt. econs; eauto. 
   Qed.
 
 
@@ -699,29 +557,16 @@ Section SIM.
         (sim_itree: forall (R_src R_tgt: Type)
                            (RR: st_local -> st_local -> R_src -> R_tgt -> Prop), bool -> bool -> world -> st_local * itree Es R_src -> st_local * itree Es R_tgt -> Prop)
         R_src R_tgt (RR: st_local -> st_local -> R_src -> R_tgt -> Prop)
-        f_src0 f_tgt0 f_src1 f_tgt1 w st_src0 st_tgt0
-        (SIM: @_sim_itree sim_itree _ _ RR f_src0 f_tgt0 w st_src0 st_tgt0)
+        f_src0 f_tgt0 f_src1 f_tgt1 w st_src st_tgt
+        (SIM: @_sim_itree sim_itree _ _ RR f_src0 f_tgt0 w st_src st_tgt)
         (SRC: f_src0 = true -> f_src1 = true)
         (TGT: f_tgt0 = true -> f_tgt1 = true)
     :
-      @_sim_itree sim_itree _ _ RR f_src1 f_tgt1 w st_src0 st_tgt0.
+      @_sim_itree sim_itree _ _ RR f_src1 f_tgt1 w st_src st_tgt.
   Proof.
     revert f_src1 f_tgt1 SRC TGT.
-    induction SIM using _sim_itree_ind2; i; clarify.
-    { econs 1; eauto. }
-    { econs 2; eauto. }
-    { econs 3; eauto. }
-    { econs 4; eauto. }
-    { econs 5; eauto. } 
-    { econs 6; eauto. } 
-    { econs 7; eauto. } 
-    { econs 8; eauto. des. esplits; eauto. }
-    { econs 9; eauto. i. exploit K; eauto. i. des. eauto. }
-    { econs 10; eauto. i. exploit K; eauto. i. des. eauto. }
-    { econs 11; eauto. des. esplits; eauto. }
-    { econs 12; eauto. }
-    { econs 13; eauto. } 
-    { exploit SRC0; auto. exploit TGT0; auto. i. clarify. econs; eauto. }
+    induction SIM; i; clarify; et.
+    { exploit SRC; auto. exploit TGT; auto. i. clarify. econs; eauto. }
   Qed.
 
 
@@ -761,66 +606,41 @@ Section SIM.
     eapply wrespect8_uclo; eauto with paco.
     econs; eauto with paco. i. inv PR.
     eapply GF in SIM.
-    revert x3 x4 SRC TGT. induction SIM using _sim_itree_ind2; i; clarify.
-    { econs 1; eauto. }
-    { econs 2; eauto. i. exploit K; eauto. i. des.
-      esplits; eauto. eapply rclo8_base. eauto. }
-    { econs 3; eauto. i. eapply rclo8_base. eauto. }
-    { econs 4; eauto. }
-    { econs 5; eauto. }
-    { econs 6; eauto. }
-    { econs 7; eauto. }
-    { econs 8; eauto.  des. esplits; eauto. }
-    { econs 9; eauto. i. exploit K; eauto. i. des. esplits; eauto. }
-    { econs 10; eauto. i. exploit K; eauto. i. des. esplits; eauto. }
-    { econs 11; eauto. des. esplits; eauto. }
-    { econs 12; eauto. }
-    { econs 13; eauto. }
-    { exploit SRC0; auto. exploit TGT0; auto. i. clarify. econs 14; eauto.
+    revert x3 x4 SRC TGT. induction SIM; i; clarify; et.
+    { exploit SRC; auto. exploit TGT; auto. i. clarify. econs 14; eauto.
       eapply rclo8_base; auto. }
   Qed.
 
-  Lemma sim_itree_flag_down  R0 R1 RR r g w st_src0 st_tgt0 f_src f_tgt
-        (SIM: gpaco8 _sim_itree (cpn8 _sim_itree) r g R0 R1 RR false false w st_src0 st_tgt0)
+  Lemma sim_itree_flag_down  R0 R1 RR r g w st_src st_tgt f_src f_tgt
+        (SIM: gpaco8 _sim_itree (cpn8 _sim_itree) r g R0 R1 RR false false w st_src st_tgt)
     :
-      gpaco8 _sim_itree (cpn8 _sim_itree) r g R0 R1 RR f_src f_tgt w st_src0 st_tgt0.
+      gpaco8 _sim_itree (cpn8 _sim_itree) r g R0 R1 RR f_src f_tgt w st_src st_tgt.
   Proof.
     guclo lflagC_spec. econs; eauto.
   Qed.
 
-  Lemma sim_itree_bot_flag_up  R0 R1 RR w st_src0 st_tgt0 f_src f_tgt
-        (SIM: paco8 _sim_itree bot8 R0 R1 RR true true w st_src0 st_tgt0)
+  Lemma sim_itree_bot_flag_up  R0 R1 RR w st_src st_tgt f_src f_tgt
+        (SIM: paco8 _sim_itree bot8 R0 R1 RR true true w st_src st_tgt)
     :
-      paco8 _sim_itree bot8 R0 R1 RR f_src f_tgt w st_src0 st_tgt0.
+      paco8 _sim_itree bot8 R0 R1 RR f_src f_tgt w st_src st_tgt.
   Proof.
     ginit. remember true in SIM at 1. remember true in SIM at 1.
-    clear Heqb Heqb0. revert w st_src0 st_tgt0 f_src f_tgt b b0 SIM.
+    clear Heqb Heqb0. revert w st_src st_tgt f_src f_tgt b b0 SIM.
     gcofix CIH. 
     i. revert f_src f_tgt.
 
     (* TODO: why induction using sim_itree_ind doesn't work? *)
-    pattern b, b0, w, st_src0, st_tgt0.
+    pattern b, b0, w, st_src, st_tgt.
     match goal with
-    | |- ?P b b0 w st_src0 st_tgt0 => set P
+    | |- ?P b b0 w st_src st_tgt => set P
     end.
-    revert b b0 w st_src0 st_tgt0 SIM.
-    eapply (@sim_itree_ind R0 R1 RR P); subst P; ss; i; clarify.
-    { guclo sim_itree_indC_spec. econs 1; eauto. }
-    { gstep. econs 2; eauto. i. gbase. eapply CIH; eauto. }
-    { gstep. econs 3; eauto. i. gbase. eapply CIH; eauto. }
-    { guclo sim_itree_indC_spec. econs 4; eauto. }
-    { guclo sim_itree_indC_spec. econs 5; eauto. } 
-    { guclo sim_itree_indC_spec. econs 6; eauto. } 
-    { guclo sim_itree_indC_spec. econs 7; eauto. } 
-    { guclo sim_itree_indC_spec. econs 8; eauto. des. esplits; eauto. }
-    { guclo sim_itree_indC_spec. econs 9; eauto. i. hexploit K; eauto. i. des. esplits; eauto. }
-    { guclo sim_itree_indC_spec. econs 10; eauto. i. hexploit K; eauto. i. des. esplits; eauto. }
-    { guclo sim_itree_indC_spec. econs 11; eauto. des. esplits; eauto. }
-    { guclo sim_itree_indC_spec. econs 12; eauto. } 
-    { guclo sim_itree_indC_spec. econs 13; eauto. } 
-    { eapply sim_itree_flag_down. gfinal. right.
-      eapply paco8_mon; eauto. ss.
-    }
+    revert b b0 w st_src st_tgt SIM.
+    eapply (@sim_itree_ind R0 R1 RR P); subst P; ss; i; clarify; try (guclo sim_itree_indC_spec; econs; et).
+    { i. gstep. econs; et. gfinal. left. et. }
+    { i. gstep. econs; et. gfinal. left. et. }
+    { i. hexploit K; eauto. i. des. esplits; eauto. }
+    { i. hexploit K; eauto. i. des. esplits; eauto. }
+    { eapply sim_itree_flag_down. gfinal. right. eapply paco8_mon; eauto. ss. }
   Qed.
 
   Variant lbindR (r s: forall S_src S_tgt (SS: st_local -> st_local -> S_src -> S_tgt -> Prop), bool -> bool -> world -> st_local * itree Es S_src -> st_local * itree Es S_tgt -> Prop):
@@ -828,15 +648,15 @@ Section SIM.
   | lbindR_intro
       f_src f_tgt w0 w1
       R_src R_tgt RR
-      (st_src0 st_tgt0: st_local)
+      (st_src st_tgt: st_local)
       (i_src: itree Es R_src) (i_tgt: itree Es R_tgt)
-      (SIM: r _ _ RR f_src f_tgt w0 (st_src0, i_src) (st_tgt0, i_tgt))
+      (SIM: r _ _ RR f_src f_tgt w0 (st_src, i_src) (st_tgt, i_tgt))
 
       S_src S_tgt SS
       (k_src: ktree Es R_src S_src) (k_tgt: ktree Es R_tgt S_tgt)
-      (SIMK: forall st_src1 st_tgt1 vret_src vret_tgt (SIM: RR st_src1 st_tgt1 vret_src vret_tgt), s _ _ SS false false w1 (st_src1, k_src vret_src) (st_tgt1, k_tgt vret_tgt))
+      (SIMK: forall st_src0 st_tgt0 vret_src vret_tgt (SIM: RR st_src0 st_tgt0 vret_src vret_tgt), s _ _ SS false false w1 (st_src0, k_src vret_src) (st_tgt0, k_tgt vret_tgt))
     :
-      lbindR r s SS f_src f_tgt w1 (st_src0, ITree.bind i_src k_src) (st_tgt0, ITree.bind i_tgt k_tgt)
+      lbindR r s SS f_src f_tgt w1 (st_src, ITree.bind i_src k_src) (st_tgt, ITree.bind i_tgt k_tgt)
   .
 
   Hint Constructors lbindR: core.
@@ -857,30 +677,16 @@ Section SIM.
     econs.
     { ii. eapply lbindR_mon; eauto. }
     i. rename l into llll. inv PR; csc.
-    remember (st_src0, i_src). remember(st_tgt0, i_tgt).
-    revert st_src0 i_src st_tgt0 i_tgt Heqp Heqp0.
+    remember (st_src, i_src). remember(st_tgt, i_tgt).
+    revert st_src i_src st_tgt i_tgt Heqp Heqp0.
     revert k_src k_tgt SIMK. eapply GF in SIM.
-    induction SIM using _sim_itree_ind2; i; clarify.
-    + rewrite ! bind_ret_l. exploit SIMK; eauto. i.
-      eapply sim_itree_flag_mon.
+    induction SIM; i; clarify; grind; try (econs; et).
+    - exploit SIMK; eauto. i.
+      eapply sim_itree_flag_mon with (f_src0 := false) (f_tgt0 := false); ss.
       { eapply sim_itree_mon; eauto. i. eapply rclo8_base. auto. }
-      { ss. }
-      { ss. }
-    + rewrite ! bind_bind. econs; eauto. i.
-      eapply rclo8_clo_base. econs; eauto.
-    + rewrite ! bind_bind. econs; eauto. i.
-      eapply rclo8_clo_base. econs; eauto.
-    + exploit IHSIM; et. i. rewrite ! bind_bind in *. econs; et. 
-    + exploit IHSIM; et. i. rewrite ! bind_bind in *. econs; et. 
-    + rewrite ! bind_tau. econs; eauto.
-    + rewrite ! bind_tau. econs; eauto.
-    + rewrite ! bind_bind. econs; eauto. des. esplits; eauto.
-    + rewrite ! bind_bind. econs; eauto. i. exploit K; eauto. i. des. esplits; eauto.
-    + rewrite ! bind_bind. econs; eauto. i. exploit K; eauto. i. des. esplits; eauto.
-    + rewrite ! bind_bind. econs; eauto. des. esplits; eauto.
-    + rewrite ! bind_bind. econs; eauto. 
-    + rewrite ! bind_bind. econs; eauto. 
-    + econs; eauto. eapply rclo8_clo_base. econs; eauto.
+    - exploit IHSIM; et. i. rewrite ! bind_bind in *. et. 
+    - exploit IHSIM; et. i. rewrite ! bind_bind in *. et. 
+    - eapply rclo8_clo_base. econs; eauto.
   Qed.
 
   Lemma lbindC_spec: lbindC  <9= gupaco8 (_sim_itree) (cpn8 (_sim_itree)).
@@ -905,8 +711,9 @@ Proof.
     eapply sim_itree_progress_flag. gbase. auto.
   }
   destruct e.
-  { dependent destruction c. rewrite <- ! bind_trigger. gstep.
-    eapply sim_itree_call; ss. ii. subst.
+  { dependent destruction c. rewrite <- ! bind_trigger.
+    gstep.
+    eapply sim_itree_call; ss. ii. subst. econs; et.
     eapply sim_itree_flag_down. gbase. auto.
   }
   destruct s.
@@ -953,9 +760,6 @@ Section SIMMODSEM.
     le: world -> world -> Prop;
     le_PreOrder: PreOrder le;
     sim_fnsems: Forall2 (sim_fnsem wf le fl_src fl_tgt) ms_src.(ModSem.fnsems) ms_tgt.(ModSem.fnsems);
-    (* sim_fnsems: forall fn f_src (FINDS: In (fn, f_src) ms_src.(ModSem.fnsems)),
-                  exists f_tgt, <<FINDT: In (fn, f_tgt) ms_tgt.(ModSem.fnsems)>>
-                                  /\ <<SIM: sim_fsem wf le ms_src.(ModSem.fnsems) ms_tgt.(ModSem.fnsems) f_src f_tgt>>; *)
     sim_initial: exists w_init, wf w_init (ms_src.(ModSem.init_st), ms_tgt.(ModSem.init_st));
   }.
 
@@ -1082,11 +886,11 @@ Section SEMPAIR.
           (<<SIM: sim_fsem wf le fl_src fl_tgt f_src f_tgt>>)).
           
   Variant g_lift_rel
-          (w0: world) st_src0 st_tgt0: Prop :=
+          (w0: world) st_src st_tgt: Prop :=
   | g_lift_rel_intro
       w1
       (LE: le w0 w1)
-      (MN: wf w1 (st_src0, st_tgt0))
+      (MN: wf w1 (st_src, st_tgt))
       
       (* (NMN: forall mn' (NIN: mn <> mn'), st_local mn' = st_local mn') *)
   .
@@ -1096,15 +900,15 @@ Section SEMPAIR.
   | my_r0_intro
       w0
       (itr_src itr_tgt: itree Es Any.t)
-      st_src0 st_tgt0 o_src o_tgt
-      (SIM: sim_itree wf le fl_src fl_tgt o_src o_tgt w0 (st_src0, itr_src) (st_tgt0, itr_tgt))
+      st_src st_tgt o_src o_tgt
+      (SIM: sim_itree wf le fl_src fl_tgt o_src o_tgt w0 (st_src, itr_src) (st_tgt, itr_tgt))
       (* (STATE: forall mn' (MN: mn <> mn'), st_local mn' = st_local mn') *)
     :
       my_r0 (fun '(st_src, ret_src) '(st_tgt, ret_tgt) =>
                 g_lift_rel w0 st_src st_tgt /\ ret_src = ret_tgt)
             o_src o_tgt
-            (interp_Es (ModSem.prog ms_src) (itr_src) st_src0)
-            (interp_Es (ModSem.prog ms_tgt) (itr_tgt) st_tgt0)
+            (interp_Es (ModSem.prog ms_src) (itr_src) st_src)
+            (interp_Es (ModSem.prog ms_tgt) (itr_tgt) st_tgt)
   .
 
   Let sim_lift: my_r0 <7= simg.
@@ -1113,10 +917,10 @@ Section SEMPAIR.
     { i. eapply cpn7_wcompat; eauto with paco. }
     gcofix CIH. i. destruct PR.
     unfold sim_itree in SIM.
-    remember (st_src0, itr_src).
-    remember (st_tgt0, itr_tgt).
+    remember (st_src, itr_src).
+    remember (st_tgt, itr_tgt).
     remember w0 in SIM at 2.
-    revert st_src0 itr_src st_tgt0 itr_tgt Heqp Heqp0 Heqw.
+    revert st_src itr_src st_tgt itr_tgt Heqp Heqp0 Heqw.
     (* TODO: why induction using sim_itree_ind doesn't work? *)
     pattern o_src, o_tgt, w, p, p0.
     match goal with
@@ -1217,7 +1021,6 @@ Definition addf f1 f2 : alist gname (Any.t -> itree _ Any.t) :=
 
 Lemma sim_ctx_aux {world}
       w wf le
-      (* ctx ms_src ms_tgt *)
       a b c
       fa fb fc 
       ol or stl str itl itr
@@ -1227,12 +1030,10 @@ Lemma sim_ctx_aux {world}
 
       (SIM: sim_itree wf le fb fc ol or w (b, itl) (c, itr))
 :
-      @sim_itree world (wf_lift wf) le (addf fb fa) (addf fc fa) ol or w (stl, translate emb_l itl) 
-                                              (str, translate emb_l itr)
-      (* @sim_itree world (wf_lift wf) le (add ctx ms_src).(fnsems) (add ctx ms_tgt).(fnsems) ol or w (stl, translate emb_r itl) 
-                                              (str, translate emb_r itr) *)
+      @sim_itree world (wf_lift wf) le (addf fb fa) (addf fc fa) ol or w (stl, translate (emb_ run_l) itl) 
+                                              (str, translate (emb_ run_l) itr)
 .
-Proof. 
+Proof.
   ginit.
 
   revert_until wf.
@@ -1254,7 +1055,7 @@ Proof.
   eapply (@sim_itree_ind world wf le fb fc Any.t Any.t (lift_rel wf le w0 (@eq Any.t)) P); subst P; ss; i; des; clarify.
 
   - rr in RET. des. clarify.
-    erewrite ! (bisimulation_is_eq _ _ (translate_ret _ _)).
+    rewrite translate_emb_ret.
     gstep. apply sim_itree_ret.
     econs; et. esplits; et.
     unfold wf_lift. rewrite SRC, TGT. split; et.
@@ -1274,155 +1075,64 @@ Proof.
     | |- ?P ol or w p p0 => set P
     end.
     eapply (@sim_itree_ind world wf le fb fc Any.t Any.t (lift_rel wf le w0 (@eq Any.t)) P); subst P; ss; i; des; clarify;
-    erewrite ! (bisimulation_is_eq _ _ (translate_bind _ _ _ )); unfold trigger; 
-    erewrite ! (bisimulation_is_eq _ _ (translate_vis _ _ _ _)); rewrite <- ! bind_trigger;
-    grind; resub; gstep; econs;
-    try (unfold wf_lift; rewrite SRC, TGT; split; auto; try (apply WF); try(apply WF0));
-    try (unfold wf_lift; rewrite SRC0, TGT0; split; auto; apply WF);
-    ii; erewrite ! (bisimulation_is_eq _ _ (translate_ret _ _));
-    grind; gfinal; left; ss; des_ifs; try (rename WF0 into WF1); inv WF1;
-    eapply CIH with (a:= t3); et; specialize (K _ vret _ _ WLE H); pclearbot; apply K.
+    rewrite ! translate_emb_bind, translate_emb_callE; gstep; econs;
+    try (match goal with
+    | |- wf_lift _ _ (_, _) =>  unfold wf_lift; rewrite SRC, TGT; et
+    end).
+    all: ii; econs; gfinal; left; ss; des_ifs; try rename WF0 into WF1; inv WF1; eapply CIH; et;
+         specialize (K _ vret _ _ WLE H); pclearbot; apply sim_itree_bot_flag_up; apply K.
     
   - punfold SIM. inv SIM; (try rewrite ! bind_trigger in H4); (try rewrite ! bind_trigger in H6); clarify.
     + apply inj_pair2 in H0, H1.
-      erewrite ! (bisimulation_is_eq _ _ (translate_bind _ _ _ )).
-      unfold trigger.
-      erewrite ! (bisimulation_is_eq _ _ (translate_vis _ _ _ _)).
-      rewrite <- ! bind_trigger.
-      grind. resub.
-      gstep; econs.
-      ii. 
-      erewrite ! (bisimulation_is_eq _ _ (translate_ret _ _)).
-      grind.
-      gfinal. left.
-      (* ss; des_ifs. inv WF1.  *)
-      eapply CIH with (a:= a); et.
-      specialize (K0 vret).
-      pclearbot. apply K0.
+      rewrite ! translate_emb_bind, translate_emb_eventE.
+      gstep. econs. i. econs. 
+      gfinal. left. eapply CIH; et.
+      apply sim_itree_bot_flag_up. pfold. apply K0. 
+
     + pclearbot. punfold SIM0. inv SIM0; (try rewrite ! bind_trigger in H4); (try rewrite ! bind_trigger in H6); clarify.
       apply inj_pair2 in H0, H1.
-      erewrite ! (bisimulation_is_eq _ _ (translate_bind _ _ _ )).
-      unfold trigger.
-      erewrite ! (bisimulation_is_eq _ _ (translate_vis _ _ _ _)).
-      rewrite <- ! bind_trigger.
-      grind. resub.
-      gstep. econs.
-      ii. 
-      erewrite ! (bisimulation_is_eq _ _ (translate_ret _ _)).
-      grind.
-      gfinal. left.
-      eapply CIH with (a:= a); et.
-      specialize (K0 vret).
-      pclearbot. apply K0.
-  - erewrite (bisimulation_is_eq _ _ (translate_bind _ _ _)).
-    unfold trigger.
-    erewrite (bisimulation_is_eq _ _ (translate_vis _ _ _ _)).
-    rewrite <- bind_trigger. grind.
+      rewrite ! translate_emb_bind, translate_emb_eventE.
+      gstep. econs. ii. econs.
+      gfinal. left. eapply CIH; et.
+      apply sim_itree_bot_flag_up. pfold. apply K0.
+
+  - rewrite ! translate_emb_bind, translate_emb_callE.
     guclo sim_itree_indC_spec.
-
-
-    (* destruct (alist_find fn fa) eqn:FA.
-    { econs; et.
-      { 
-        unfold addf. rewrite alist_find_app_o.
-        unfold trans_l, trans_r. rewrite ! alist_find_map. unfold o_map.
-        rewrite FA. et.
-      }
-    } *)
-
-
-    
     econs; et.
     { 
       unfold addf. apply alist_find_app.
       unfold trans_l. rewrite alist_find_map. unfold o_map.
       rewrite FUN. et.
     }
-
-    ss. rewrite <- bind_bind.
-    erewrite <- ! (bisimulation_is_eq _ _ (translate_bind _ _ _)).
-    eapply IH; et. f_equal. grind. f_equal.
-    apply func_ext. i.
-    rewrite bind_ret_l. et.
-  - erewrite (bisimulation_is_eq _ _ (translate_bind _ _ _)).
-    unfold trigger.
-    erewrite (bisimulation_is_eq _ _ (translate_vis _ _ _ _)).
-    rewrite <- bind_trigger. grind.
+    ss. rewrite <- ! translate_emb_bind.
+    eapply IH; et. 
+  - rewrite ! translate_emb_bind, translate_emb_callE.
     guclo sim_itree_indC_spec. econs; et.
     { unfold addf. apply alist_find_app. unfold trans_l. rewrite alist_find_map. unfold o_map. rewrite FUN. et. }
-    ss. rewrite <- bind_bind.
-    erewrite <- ! (bisimulation_is_eq _ _ (translate_bind _ _ _)).
-    eapply IH; et. f_equal. grind. f_equal.
-    apply func_ext. i.
-    rewrite bind_ret_l. et.
-  - erewrite ! (bisimulation_is_eq _ _ (translate_tau _ _)).
+    ss. rewrite <- ! translate_emb_bind.
+    eapply IH; et. 
+  - rewrite ! translate_emb_tau. 
     guclo sim_itree_indC_spec. econs; et.
-  - erewrite ! (bisimulation_is_eq _ _ (translate_tau _ _)).
+  - rewrite ! translate_emb_tau. 
+    guclo sim_itree_indC_spec. econs; et.    
+  - rewrite ! translate_emb_bind, translate_emb_eventE.
     guclo sim_itree_indC_spec. econs; et.
-  - erewrite ! (bisimulation_is_eq _ _ (translate_bind _ _ _)).
-    unfold trigger.
-    erewrite ! (bisimulation_is_eq _ _ (translate_vis _ _ _ _)).
-    rewrite <- ! bind_trigger.
-    grind. 
+  - rewrite ! translate_emb_bind, translate_emb_eventE.
     guclo sim_itree_indC_spec. econs; et.
-    exists x.
-    erewrite ! (bisimulation_is_eq _ _ (translate_ret _ _)).
-    rewrite bind_ret_l.
-    et.
-  - erewrite ! (bisimulation_is_eq _ _ (translate_bind _ _ _)).
-    unfold trigger.
-    erewrite ! (bisimulation_is_eq _ _ (translate_vis _ _ _ _)).
-    rewrite <- ! bind_trigger.
-    grind.
+    i. specialize (K x). des. et.
+  - rewrite ! translate_emb_bind, translate_emb_eventE.
     guclo sim_itree_indC_spec. econs; et.
-    i.
-    erewrite ! (bisimulation_is_eq _ _ (translate_ret _ _)).
-    rewrite bind_ret_l.
-    specialize (K x). des. et.
-  - erewrite ! (bisimulation_is_eq _ _ (translate_bind _ _ _)).
-    unfold trigger.
-    erewrite ! (bisimulation_is_eq _ _ (translate_vis _ _ _ _)).
-    rewrite <- ! bind_trigger.
-    grind.
+    i. specialize (K x). des. et.    
+  - rewrite ! translate_emb_bind, translate_emb_eventE.
     guclo sim_itree_indC_spec. econs; et.
-    i.
-    erewrite ! (bisimulation_is_eq _ _ (translate_ret _ _)).
-    rewrite bind_ret_l.
-    specialize (K x). des. et.    
-  - erewrite ! (bisimulation_is_eq _ _ (translate_bind _ _ _)).
-    unfold trigger.
-    erewrite ! (bisimulation_is_eq _ _ (translate_vis _ _ _ _)).
-    rewrite <- ! bind_trigger.
-    grind. 
+  - rewrite ! translate_emb_bind, translate_emb_sE.
     guclo sim_itree_indC_spec. econs; et.
-    exists x.
-    erewrite ! (bisimulation_is_eq _ _ (translate_ret _ _)).
-    rewrite bind_ret_l.
-    et.
-  - erewrite ! (bisimulation_is_eq _ _ (translate_bind _ _ _)).
-    unfold trigger.
-    erewrite ! (bisimulation_is_eq _ _ (translate_vis _ _ _ _)).
-    rewrite <- ! bind_trigger.
-    grind. resub. 
+    unfold run_l. rewrite SRC. des_ifs; ss. 
+    eapply IH; et. rewrite Any.pair_split; et.
+  - rewrite ! translate_emb_bind, translate_emb_sE.
     guclo sim_itree_indC_spec. econs; et.
-    erewrite ! (bisimulation_is_eq _ _ (translate_ret _ _)).
-    rewrite bind_ret_l.
-    unfold run_l. rewrite SRC.
-    des_ifs; ss.
-    eapply IH; et.
-    rewrite Any.pair_split. et.
-  - erewrite ! (bisimulation_is_eq _ _ (translate_bind _ _ _)).
-    unfold trigger.
-    erewrite ! (bisimulation_is_eq _ _ (translate_vis _ _ _ _)).
-    rewrite <- ! bind_trigger.
-    grind. resub. 
-    guclo sim_itree_indC_spec. econs; et.
-    erewrite ! (bisimulation_is_eq _ _ (translate_ret _ _)).
-    rewrite bind_ret_l.
-    unfold run_l. rewrite TGT.
-    des_ifs; ss.
-    eapply IH; et.
-    rewrite Any.pair_split. et.   
+    unfold run_l. rewrite TGT. des_ifs; ss. 
+    eapply IH; et. rewrite Any.pair_split; et. 
   - remember (true) as o_src.
     remember (true) as o_tgt.
     rewrite Heqo_src at 2.
@@ -1435,17 +1145,17 @@ Proof.
     unfold sim_itree in SIM0'.
     rewrite Weq in SIM0' at 2.
 
-    revert a b c stl str itl itr SRC0 TGT0 PL PR Weq Heqo_src Heqo_tgt SIM0.
+    revert a b c stl str itl itr SRC TGT PL PR Weq Heqo_src Heqo_tgt SIM0.
     pattern o_src, o_tgt, w1, p1, p2.
     match goal with
     | |- ?P o_src o_tgt w1 p1 p2 => set P
     end.
     eapply (@sim_itree_ind world wf le fb fc Any.t Any.t (lift_rel wf le w0 (@eq Any.t)) P); subst P; ss; i; des; clarify.
     + rr in RET. des. clarify.
-      erewrite ! (bisimulation_is_eq _ _ (translate_ret _ _)).
+      rewrite ! translate_emb_ret.
       gstep. apply sim_itree_ret.
       econs; et. esplits; et.
-      unfold wf_lift. rewrite SRC0, TGT0. split; et.
+      unfold wf_lift. rewrite SRC, TGT. split; et.
     + remember (` x : _ <- trigger (Call fn varg);; k_src x). 
       remember (` x : _ <- trigger (Call fn varg);; k_tgt x). 
       remember (b, ` x : _ <- trigger (Call fn varg);; k_src x) eqn:PL.
@@ -1455,140 +1165,64 @@ Proof.
       unfold sim_itree in SIM''.
       rewrite Weq in SIM'' at 2.
 
-      revert a b c stl str i i0 WF SRC0 TGT0 PL PR Weq SIM SIM0 SIM'' Heqi Heqi0.
+      revert a b c stl str i i0 WF SRC TGT PL PR Weq SIM SIM0 SIM'' Heqi Heqi0.
       pattern ol, or, w, p, p0.
       match goal with
       | |- ?P ol or w p p0 => set P
       end.
       eapply (@sim_itree_ind world wf le fb fc Any.t Any.t (lift_rel wf le w0 (@eq Any.t)) P); subst P; ss; i; des; clarify;
-      erewrite ! (bisimulation_is_eq _ _ (translate_bind _ _ _ )); unfold trigger; 
-      erewrite ! (bisimulation_is_eq _ _ (translate_vis _ _ _ _)); rewrite <- ! bind_trigger;
-      grind; resub; gstep; econs;
-      try (unfold wf_lift; rewrite SRC0, TGT0; split; auto; try (apply WF); try(apply WF0));
-      (* try (unfold wf_lift; rewrite SRC0, TGT0; split; auto; apply WF); *)
-      ii; erewrite ! (bisimulation_is_eq _ _ (translate_ret _ _));
-      grind; gfinal; left; ss; des_ifs; try (rename WF0 into WF1); inv WF1;
-      eapply CIH with (a:= t3); et; specialize (K _ vret _ _ WLE H); pclearbot; apply K.
+      rewrite ! translate_emb_bind, translate_emb_callE; gstep; econs; 
+      try (match goal with 
+          | |- wf_lift _ _ _ => unfold wf_lift; rewrite SRC, TGT; et
+          end
+      ).
+      all: ii; econs; gfinal; left; ss; des_ifs; try rename WF0 into WF1; inv WF1; eapply CIH; et;
+      specialize (K _ vret _ _ WLE H); pclearbot; apply sim_itree_bot_flag_up; apply K.
     + punfold SIM0. inv SIM0; (try rewrite ! bind_trigger in H4); (try rewrite ! bind_trigger in H6); clarify.
       * apply inj_pair2 in H0, H1.
-        erewrite ! (bisimulation_is_eq _ _ (translate_bind _ _ _ )).
-        unfold trigger.
-        erewrite ! (bisimulation_is_eq _ _ (translate_vis _ _ _ _)).
-        rewrite <- ! bind_trigger.
-        grind. resub.
-        gstep; econs.
-        ii. 
-        erewrite ! (bisimulation_is_eq _ _ (translate_ret _ _)).
-        grind.
-        gfinal. left.
-        eapply CIH with (a:= a); et.
-        specialize (K0 vret).
-        pclearbot. apply K0.
+        rewrite ! translate_emb_bind, translate_emb_eventE.
+        gstep. econs. i. econs.
+        gfinal. left. eapply CIH; et.
+        apply sim_itree_bot_flag_up. pfold. eapply K0.
+
       * pclearbot. punfold SIM1. inv SIM1; (try rewrite ! bind_trigger in H4); (try rewrite ! bind_trigger in H6); clarify.
         apply inj_pair2 in H0, H1.
-        erewrite ! (bisimulation_is_eq _ _ (translate_bind _ _ _ )).
-        unfold trigger.
-        erewrite ! (bisimulation_is_eq _ _ (translate_vis _ _ _ _)).
-        rewrite <- ! bind_trigger.
-        grind. resub.
-        gstep. econs.
-        ii. 
-        erewrite ! (bisimulation_is_eq _ _ (translate_ret _ _)).
-        grind.
-        gfinal. left.
-        eapply CIH with (a:= a); et.
-        specialize (K0 vret).
-        pclearbot. apply K0.
-    + erewrite (bisimulation_is_eq _ _ (translate_bind _ _ _)).
-      unfold trigger.
-      erewrite (bisimulation_is_eq _ _ (translate_vis _ _ _ _)).
-      rewrite <- bind_trigger. grind.
+        rewrite ! translate_emb_bind, translate_emb_eventE.
+        gstep. econs. i. econs.
+        gfinal. left. eapply CIH; et.
+        apply sim_itree_bot_flag_up. pfold. eapply K0.
+    + rewrite ! translate_emb_bind, translate_emb_callE.
       guclo sim_itree_indC_spec. econs; et.
       { unfold addf. apply alist_find_app. unfold trans_l. rewrite alist_find_map. unfold o_map. rewrite FUN. et. }
-      ss. rewrite <- bind_bind.
-      erewrite <- ! (bisimulation_is_eq _ _ (translate_bind _ _ _)).
-      eapply IH; et. f_equal. grind. f_equal.
-      apply func_ext. i.
-      rewrite bind_ret_l. et.
-    + erewrite (bisimulation_is_eq _ _ (translate_bind _ _ _)).
-      unfold trigger.
-      erewrite (bisimulation_is_eq _ _ (translate_vis _ _ _ _)).
-      rewrite <- bind_trigger. grind.
+      ss. rewrite <- ! translate_emb_bind.
+      eapply IH; et.
+    + rewrite ! translate_emb_bind, translate_emb_callE.
       guclo sim_itree_indC_spec. econs; et.
       { unfold addf. apply alist_find_app. unfold trans_l. rewrite alist_find_map. unfold o_map. rewrite FUN. et. }
-      ss. rewrite <- bind_bind.
-      erewrite <- ! (bisimulation_is_eq _ _ (translate_bind _ _ _)).
-      eapply IH; et. f_equal. grind. f_equal.
-      apply func_ext. i.
-      rewrite bind_ret_l. et.
-    + erewrite ! (bisimulation_is_eq _ _ (translate_tau _ _)).
+      ss. rewrite <- ! translate_emb_bind.
+      eapply IH; et.
+    + rewrite ! translate_emb_tau. 
       guclo sim_itree_indC_spec. econs. et. 
-    + erewrite ! (bisimulation_is_eq _ _ (translate_tau _ _)).
+    + rewrite ! translate_emb_tau. 
+      guclo sim_itree_indC_spec. econs. et. 
+    + rewrite ! translate_emb_bind, translate_emb_eventE.
+      guclo sim_itree_indC_spec. econs. et.
+    + rewrite! translate_emb_bind, translate_emb_eventE.
+      guclo sim_itree_indC_spec. econs. et.
+      i. specialize (K x). des. et.
+    + rewrite! translate_emb_bind, translate_emb_eventE.
+      guclo sim_itree_indC_spec. econs. et.
+      i. specialize (K x). des. et.    
+    + rewrite ! translate_emb_bind, translate_emb_eventE.
+      guclo sim_itree_indC_spec. econs. et.
+    + rewrite ! translate_emb_bind, translate_emb_sE.
       guclo sim_itree_indC_spec. econs; et.
-    + erewrite ! (bisimulation_is_eq _ _ (translate_bind _ _ _)).
-      unfold trigger.
-      erewrite ! (bisimulation_is_eq _ _ (translate_vis _ _ _ _)).
-      rewrite <- ! bind_trigger.
-      grind. 
+      unfold run_l. rewrite SRC. des_ifs; ss.
+      eapply IH; et. rewrite Any.pair_split. et.
+    + rewrite ! translate_emb_bind, translate_emb_sE.
       guclo sim_itree_indC_spec. econs; et.
-      exists x.
-      erewrite ! (bisimulation_is_eq _ _ (translate_ret _ _)).
-      rewrite bind_ret_l.
-      et.
-    + erewrite ! (bisimulation_is_eq _ _ (translate_bind _ _ _)).
-      unfold trigger.
-      erewrite ! (bisimulation_is_eq _ _ (translate_vis _ _ _ _)).
-      rewrite <- ! bind_trigger.
-      grind.
-      guclo sim_itree_indC_spec. econs; et.
-      i.
-      erewrite ! (bisimulation_is_eq _ _ (translate_ret _ _)).
-      rewrite bind_ret_l.
-      specialize (K x). des. et.
-    + erewrite ! (bisimulation_is_eq _ _ (translate_bind _ _ _)).
-      unfold trigger.
-      erewrite ! (bisimulation_is_eq _ _ (translate_vis _ _ _ _)).
-      rewrite <- ! bind_trigger.
-      grind.
-      guclo sim_itree_indC_spec. econs; et.
-      i.
-      erewrite ! (bisimulation_is_eq _ _ (translate_ret _ _)).
-      rewrite bind_ret_l.
-      specialize (K x). des. et.    
-    + erewrite ! (bisimulation_is_eq _ _ (translate_bind _ _ _)).
-      unfold trigger.
-      erewrite ! (bisimulation_is_eq _ _ (translate_vis _ _ _ _)).
-      rewrite <- ! bind_trigger.
-      grind. 
-      guclo sim_itree_indC_spec. econs; et.
-      exists x.
-      erewrite ! (bisimulation_is_eq _ _ (translate_ret _ _)).
-      rewrite bind_ret_l.
-      et.
-    + erewrite ! (bisimulation_is_eq _ _ (translate_bind _ _ _)).
-      unfold trigger.
-      erewrite ! (bisimulation_is_eq _ _ (translate_vis _ _ _ _)).
-      rewrite <- ! bind_trigger.
-      grind. resub. 
-      guclo sim_itree_indC_spec. econs; et.
-      erewrite ! (bisimulation_is_eq _ _ (translate_ret _ _)).
-      rewrite bind_ret_l.
-      unfold run_l. rewrite SRC0.
-      des_ifs; ss.
-      eapply IH; et.
-      rewrite Any.pair_split. et.
-    + erewrite ! (bisimulation_is_eq _ _ (translate_bind _ _ _)).
-      unfold trigger.
-      erewrite ! (bisimulation_is_eq _ _ (translate_vis _ _ _ _)).
-      rewrite <- ! bind_trigger.
-      grind. resub. 
-      guclo sim_itree_indC_spec. econs; et.
-      erewrite ! (bisimulation_is_eq _ _ (translate_ret _ _)).
-      rewrite bind_ret_l.
-      unfold run_l. rewrite TGT0.
-      des_ifs; ss.
-      eapply IH; et.
-      rewrite Any.pair_split. et.   
+      unfold run_l. rewrite TGT. des_ifs; ss.
+      eapply IH; et. rewrite Any.pair_split. et.      
     + gstep. econs; et.
       gfinal. left. eapply CIH; et.
 Qed.
@@ -1604,8 +1238,6 @@ Proof.
   econs; et.
   2: { exists x. instantiate (1:= wf_lift wf0). s.
        rewrite ! Any.pair_split.
-       (* exists (fun _ => fun '(stl, str) => stl = str). *)
-       (* exists wf0. *)
        splits; et.
   }
   s. unfold add_fnsems, trans_l, trans_r.
@@ -1616,11 +1248,9 @@ Proof.
     destruct (Any.split mrs_src) eqn: SRC; destruct (Any.split mrs_tgt) eqn:TGT; clarify.
     2: { destruct p. clarify. }
     destruct p, p0. des. clarify.
-    (* assert (exists w1, le w w1 /\ wf1 w1 (t0, t2) /\ wf2 w1 (t1, t3)). *)
     assert (exists w1, le w w1 /\ wf0 w1 (t0, t2)).
     { exists w. splits; et. refl. }
     clear SIMMRS.
-    (* clear SIMMRS SIMMRS0. *)
     des.
     ginit.
     revert_until w1.
@@ -1629,30 +1259,23 @@ Proof.
     revert SRC TGT.
     revert t0 t2 t3.
     revert mrs_src mrs_tgt.
-    (* revert wf1 wf2. *)
     
     generalize (i y) as it.
     revert_until wf0.
-    (* revert w. *)
-    (* revert SIMMRS SIMMRS0. *)
-    (* revert t0 t1 t2 t3. *)
-    (* revert wf1 wf2. *)
     gcofix CIH. i.
     apply Any.split_pair in SRC. 
     apply Any.split_pair in TGT.
     des. clarify.  
     ides it.
-    + erewrite ! (bisimulation_is_eq _ _ (translate_ret _ _)).
+    + rewrite ! translate_emb_ret.
       gstep. apply sim_itree_ret.
-      unfold lift_rel. 
-      esplits; et.
+      unfold lift_rel. esplits; et.
       s. rewrite ! Any.pair_split. et.     
-    + erewrite ! (bisimulation_is_eq _ _ (translate_tau _ _)).
+    + rewrite ! translate_emb_tau.
       gstep. 
       apply sim_itree_tau_src. apply sim_itree_tau_tgt. 
       eapply sim_itree_progress; et.
       gfinal. left. 
-      (* eapply CIH with (t0 := t0); et; des; clarify; rewrite ! Any.pair_split; et. *)
       eapply CIH; et; des; clarify; rewrite ! Any.pair_split; et.
     + erewrite ! (bisimulation_is_eq _ _ (translate_vis _ _ _ _)).
       rewrite <- ! bind_trigger.
@@ -1660,41 +1283,33 @@ Proof.
       * (* callE *)
         gstep. destruct c.
         eapply sim_itree_call; clarify.
-        { s. rewrite ! Any.pair_split.
-          (* exists wf1, wf2. et.  *)
-          (* exists wf1. et. *)
-          esplits; et. }
-        i. gstep. econs; et. gfinal. left.
-        ss. destruct (Any.split st_src1) eqn: SPL1; destruct (Any.split st_tgt1) eqn: SPL2; clarify.
+        { s. rewrite ! Any.pair_split. esplits; et. }
+        i. econs. gfinal. left.
+        ss. destruct (Any.split st_src0) eqn: SPL1; destruct (Any.split st_tgt0) eqn: SPL2; clarify.
         2: { destruct p. clarify. }
         destruct p, p0, WF.
         eapply CIH.
         9: { etrans; et. }
         all: clarify; et. 
-
       * (* sE *)
          gstep. destruct s'.
          apply sim_itree_supdate_src. apply sim_itree_supdate_tgt.
          eapply sim_itree_progress; et.
          unfold ModSem.run_r. rewrite ! Any.pair_split.
          gfinal. left. destruct (run t3). ss. eapply CIH; et; rewrite ! Any.pair_split; et.
-      
       * (* eventE *)
         gstep. destruct e'.
-        (* Choose *)
-        -- apply sim_itree_choose_tgt. i. apply sim_itree_choose_src. exists x0.
+        -- (* Choose *)
+           apply sim_itree_choose_tgt. i. eapply sim_itree_choose_src.
            eapply sim_itree_progress; et.
            gfinal. left. eapply CIH; et; rewrite ! Any.pair_split; et.
-        (* Take *)
-        -- apply sim_itree_take_src. i. apply sim_itree_take_tgt. exists x0.
+        -- (* Take *)
+           apply sim_itree_take_src. i. eapply sim_itree_take_tgt. 
            eapply sim_itree_progress; et.
            gfinal. left. eapply CIH; et; rewrite ! Any.pair_split; et.
-        (* Syscall *)
-        -- apply sim_itree_syscall. i.
-           eapply sim_itree_flag_down.
+        -- (* Syscall *)
+           apply sim_itree_syscall. i. econs.
            gfinal. left. eapply CIH; et; rewrite ! Any.pair_split; et.
-  
-
   - i. destruct H0. r in H0. rr in H1. 
     destruct a, b. econs; et. ss.
     ii; clarify. ss. 
