proofmode/HPSim.v
@@ -14,6 +14,7 @@ From ExtLib Require Import
      Data.Map.FMapAList.
 Require Import Red IRed.
 Require Import ProofMode Invariant.
+Require Import HTactics.
 
 
 
@@ -37,21 +38,21 @@ Section SIM.
 	Variable fl_src: alist gname (Any.t -> itree hAGEs Any.t).
 	Variable fl_tgt: alist gname (Any.t -> itree hAGEs Any.t).
 	Variable I: Any.t -> Any.t -> iProp.
-  Variable R_src R_tgt: Type.
-  Variable Q: Any.t -> Any.t -> R_src -> R_tgt -> iProp.
-  (* Variable Q: R_src -> R_tgt -> Prop. *)
+  (* Variable Any.t Any.t: Type. *)
   
   (* Print iProp.
   Print URA.t. *)
 	(* Print current_iProp. *)
 
+
+	
 	Inductive _hpsim
-	(hpsim: bool -> bool -> Any.t * itree hAGEs R_src -> Any.t * itree hAGEs R_tgt -> Σ -> Prop)
-		: bool -> bool -> Any.t * itree hAGEs R_src -> Any.t * itree hAGEs R_tgt -> Σ -> Prop :=
+	(hpsim: bool -> bool -> Any.t * itree hAGEs Any.t -> Any.t * itree hAGEs Any.t -> Σ -> Prop)
+		: bool -> bool -> Any.t * itree hAGEs Any.t -> Any.t * itree hAGEs Any.t -> Σ -> Prop :=
 	| hpsim_ret
 			f_src f_tgt st_src st_tgt fmr
 			v_src v_tgt
-			(RET: current_iProp fmr (I st_src st_tgt ** Q st_src st_tgt v_src v_tgt))
+			(RET: current_iProp fmr (I st_src st_tgt))
 		:
 			_hpsim hpsim f_src f_tgt (st_src, Ret v_src) (st_tgt, Ret v_tgt) fmr
 
@@ -61,7 +62,7 @@ Section SIM.
       (INV: current_iProp fmr (I st_src st_tgt ** FR))
 			(K: forall vret st_src0 st_tgt0 fmr0
           (INV: current_iProp fmr0 (I st_src0 st_tgt0 ** FR)),
-				_hpsim hpsim true true (st_src0, k_src vret) (st_tgt0, k_tgt vret) fmr0)
+				_hpsim hpsim true true (st_src0, k_src vret) (st_tgt0, k_tgt vret) fmr0)				
 		:
 			_hpsim hpsim f_src f_tgt (st_src, trigger (Call fn varg) >>= k_src) (st_tgt, trigger (Call fn varg) >>= k_tgt) fmr
 
@@ -151,39 +152,39 @@ Section SIM.
 
 	| hpsim_assume_src
 			f_src f_tgt st_src st_tgt fmr
-			P k_src i_tgt FMR
+			iP k_src i_tgt FMR
       (CUR: current_iProp fmr FMR)
-			(K: forall fmr0 (NEW: current_iProp fmr0 (P ** FMR)),
+			(K: forall fmr0 (NEW: current_iProp fmr0 (iP ** FMR)),
           _hpsim hpsim true f_tgt (st_src, k_src tt) (st_tgt, i_tgt) fmr0)
 		:
-			_hpsim hpsim f_src f_tgt (st_src, trigger (Assume P) >>= k_src) (st_tgt, i_tgt) fmr
+			_hpsim hpsim f_src f_tgt (st_src, trigger (Assume iP) >>= k_src) (st_tgt, i_tgt) fmr
 
 	| hpsim_assume_tgt
 			f_src f_tgt st_src st_tgt fmr
-			P i_src k_tgt FMR
-      (CUR: current_iProp fmr (P ** FMR))
+			iP i_src k_tgt FMR
+      (CUR: current_iProp fmr (iP ** FMR))
 			(K: forall fmr0 (NEW: current_iProp fmr0 FMR),
           _hpsim hpsim f_src true (st_src, i_src) (st_tgt, k_tgt tt) fmr0)
 		:
-			_hpsim hpsim f_src f_tgt (st_src, i_src) (st_tgt, trigger (Assume P) >>= k_tgt) fmr
+			_hpsim hpsim f_src f_tgt (st_src, i_src) (st_tgt, trigger (Assume iP) >>= k_tgt) fmr
 
 	| hpsim_guarantee_src
 			f_src f_tgt st_src st_tgt fmr
-			P k_src i_tgt FMR
-      (CUR: current_iProp fmr (P ** FMR))
+			iP k_src i_tgt FMR
+      (CUR: current_iProp fmr (iP ** FMR))
 			(K: forall fmr0 (NEW: current_iProp fmr0 FMR),
           _hpsim hpsim true f_tgt (st_src, k_src tt) (st_tgt, i_tgt) fmr0)
 		:
-			_hpsim hpsim f_src f_tgt (st_src, trigger (Guarantee P) >>= k_src) (st_tgt, i_tgt) fmr
+			_hpsim hpsim f_src f_tgt (st_src, trigger (Guarantee iP) >>= k_src) (st_tgt, i_tgt) fmr
 
 	| hpsim_guarantee_tgt
 			f_src f_tgt st_src st_tgt fmr
-			P i_src k_tgt FMR
+			iP i_src k_tgt FMR
       (CUR: current_iProp fmr FMR)
-			(K: forall fmr0 (NEW: current_iProp fmr0 (P ** FMR)),
+			(K: forall fmr0 (NEW: current_iProp fmr0 (iP ** FMR)),
           _hpsim hpsim f_src true (st_src, i_src) (st_tgt, k_tgt tt) fmr0)
 		:
-			_hpsim hpsim f_src f_tgt (st_src, i_src) (st_tgt, trigger (Guarantee P) >>= k_tgt) fmr
+			_hpsim hpsim f_src f_tgt (st_src, i_src) (st_tgt, trigger (Guarantee iP) >>= k_tgt) fmr
 
 	| hpsim_progress
   		st_src st_tgt fmr
@@ -193,18 +194,400 @@ Section SIM.
   		_hpsim hpsim true true (st_src, i_src) (st_tgt, i_tgt) fmr
 	.
 
+	Lemma _hpsim_ind2
+				(hpsim: bool -> bool -> Any.t * itree hAGEs Any.t -> Any.t * itree hAGEs Any.t -> Σ -> Prop)
+				(P: bool -> bool -> Any.t * itree hAGEs Any.t -> Any.t * itree hAGEs Any.t -> Σ -> Prop)
+				(RET: forall
+						f_src f_tgt st_src st_tgt fmr
+						v_src v_tgt
+						(RET: current_iProp fmr (I st_src st_tgt)),
+						P f_src f_tgt (st_src, Ret v_src) (st_tgt, Ret v_tgt) fmr)
+				(CALL: forall
+						f_src f_tgt st_src st_tgt fmr
+						fn varg k_src k_tgt FR
+						(INV: current_iProp fmr (I st_src st_tgt ** FR))
+						(K: forall vret st_src0 st_tgt0 fmr0
+								(INV: current_iProp fmr0 (I st_src0 st_tgt0 ** FR)),
+								<<SIM: _hpsim hpsim true true (st_src0, k_src vret) (st_tgt0, k_tgt vret) fmr0>> /\
+								<<IH: P true true (st_src0, k_src vret) (st_tgt0, k_tgt vret) fmr0>>),
+						P f_src f_tgt (st_src, trigger (Call fn varg) >>= k_src) (st_tgt, trigger (Call fn varg) >>= k_tgt) fmr)
+				(SYSCALL: forall
+						f_src f_tgt st_src st_tgt fmr
+						fn varg rvs k_src k_tgt
+						(K: forall vret,
+								<<SIM: _hpsim hpsim true true (st_src, k_src vret) (st_tgt, k_tgt vret) fmr>> /\
+								<<IH: P true true (st_src, k_src vret) (st_tgt, k_tgt vret) fmr>>),
+						P f_src f_tgt (st_src, trigger (Syscall fn varg rvs) >>= k_src) (st_tgt, trigger (Syscall fn varg rvs) >>= k_tgt) fmr)
+				(INLINESRC: forall
+						f_src f_tgt st_src st_tgt fmr
+						fn f varg k_src i_tgt
+						(FUN: alist_find fn fl_src = Some f)
+						(K: _hpsim hpsim true f_tgt (st_src, (f varg) >>= k_src) (st_tgt, i_tgt) fmr)
+						(IH: P true f_tgt (st_src, (f varg) >>= k_src) (st_tgt, i_tgt) fmr),
+						P f_src f_tgt (st_src, trigger (Call fn varg) >>= k_src) (st_tgt, i_tgt) fmr)
+				(INLINETGT: forall
+						f_src f_tgt st_src st_tgt fmr
+						fn f varg i_src k_tgt
+						(FUN: alist_find fn fl_tgt = Some f)
+						(K: _hpsim hpsim f_src true (st_src, i_src) (st_tgt, (f varg) >>= k_tgt) fmr)
+						(IH: P f_src true (st_src, i_src) (st_tgt, (f varg) >>= k_tgt) fmr),
+						P f_src f_tgt (st_src, i_src) (st_tgt, trigger (Call fn varg) >>= k_tgt) fmr)
+				(TAUSRC: forall
+						f_src f_tgt st_src st_tgt fmr
+						i_src i_tgt
+						(K: _hpsim hpsim true f_tgt (st_src, i_src) (st_tgt, i_tgt) fmr)
+						(IH: P true f_tgt (st_src, i_src) (st_tgt, i_tgt) fmr),
+						P f_src f_tgt (st_src, tau;; i_src) (st_tgt, i_tgt) fmr)
+				(TAUTGT: forall
+						f_src f_tgt st_src st_tgt fmr
+						i_src i_tgt
+						(K: _hpsim hpsim f_src true (st_src, i_src) (st_tgt, i_tgt) fmr)
+						(IH: P f_src true (st_src, i_src) (st_tgt, i_tgt) fmr),
+						P f_src f_tgt (st_src, i_src) (st_tgt, tau;; i_tgt) fmr)
+				(CHOOSESRC: forall
+						f_src f_tgt st_src st_tgt fmr
+						X x k_src i_tgt
+						(K: _hpsim hpsim true f_tgt (st_src, k_src x) (st_tgt, i_tgt) fmr)
+						(IH: P true f_tgt (st_src, k_src x) (st_tgt, i_tgt) fmr),
+						P f_src f_tgt (st_src, trigger (Choose X) >>= k_src) (st_tgt, i_tgt) fmr)
+				(CHOOSETGT: forall
+						f_src f_tgt st_src st_tgt fmr
+						X i_src k_tgt
+						(K: forall (x: X), 
+								<<SIM: _hpsim hpsim f_src true (st_src, i_src) (st_tgt, k_tgt x) fmr>> /\
+								<<IH: P f_src true (st_src, i_src) (st_tgt, k_tgt x) fmr>>),
+						P f_src f_tgt (st_src, i_src) (st_tgt, trigger (Choose X) >>= k_tgt) fmr)
+				(TAKESRC: forall
+						f_src f_tgt st_src st_tgt fmr
+						X k_src i_tgt
+						(K: forall (x: X), 
+								<<SIM: _hpsim hpsim true f_tgt (st_src, k_src x) (st_tgt, i_tgt) fmr>> /\ 
+								<<IH: P true f_tgt (st_src, k_src x) (st_tgt, i_tgt) fmr>>),
+						P f_src f_tgt (st_src, trigger (Take X) >>= k_src) (st_tgt, i_tgt) fmr)
+				(TAKETGT: forall
+						f_src f_tgt st_src st_tgt fmr
+						X x i_src k_tgt
+						(K: _hpsim hpsim f_src true (st_src, i_src) (st_tgt, k_tgt x) fmr)
+						(IH: P f_src true (st_src, i_src) (st_tgt, k_tgt x) fmr),
+						P f_src f_tgt (st_src, i_src) (st_tgt, trigger (Take X) >>= k_tgt) fmr)
+				(SUPDATESRC: forall
+						f_src f_tgt st_src st_tgt fmr
+						X x st_src0 k_src i_tgt
+						(run: Any.t -> Any.t * X)
+						(RUN: run st_src = (st_src0, x))
+						(K: _hpsim hpsim true f_tgt (st_src0, k_src x) (st_tgt, i_tgt) fmr)
+						(IH: P true f_tgt (st_src0, k_src x) (st_tgt, i_tgt) fmr),
+						P f_src f_tgt (st_src, trigger (SUpdate run) >>= k_src) (st_tgt, i_tgt) fmr)
+				(SUPDATETGT: forall
+						f_src f_tgt st_src st_tgt fmr
+						X x st_tgt0 i_src k_tgt
+						(run: Any.t -> Any.t * X)
+						(RUN: run st_tgt = (st_tgt0, x))
+						(K: _hpsim hpsim f_src true (st_src, i_src) (st_tgt0, k_tgt x) fmr)
+						(IH: P f_src true (st_src, i_src) (st_tgt0, k_tgt x) fmr),
+						P f_src f_tgt (st_src, i_src) (st_tgt, trigger (SUpdate run) >>= k_tgt) fmr)
+				(ASSUMESRC: forall
+						f_src f_tgt st_src st_tgt fmr
+						iP k_src i_tgt FMR
+						(CUR: current_iProp fmr FMR)
+						(K: forall fmr0 (NEW: current_iProp fmr0 (iP ** FMR)),
+								<<SIM: _hpsim hpsim true f_tgt (st_src, k_src tt) (st_tgt, i_tgt) fmr0>> /\
+								<<IH: P true f_tgt (st_src, k_src tt) (st_tgt, i_tgt) fmr0>>),
+						P f_src f_tgt (st_src, trigger (Assume iP) >>= k_src) (st_tgt, i_tgt) fmr)
+				(ASSUMETGT: forall
+						f_src f_tgt st_src st_tgt fmr
+						iP i_src k_tgt FMR
+						(CUR: current_iProp fmr (iP ** FMR))
+						(K: forall fmr0 (NEW: current_iProp fmr0 FMR),
+								<<SIM: _hpsim hpsim f_src true (st_src, i_src) (st_tgt, k_tgt tt) fmr0>> /\
+								<<IH: P f_src true (st_src, i_src) (st_tgt, k_tgt tt) fmr0>>),
+						P f_src f_tgt (st_src, i_src) (st_tgt, trigger (Assume iP) >>= k_tgt) fmr)
+				(GUARANTEESRC: forall
+						f_src f_tgt st_src st_tgt fmr
+						iP k_src i_tgt FMR
+						(CUR: current_iProp fmr (iP ** FMR))
+						(K: forall fmr0 (NEW: current_iProp fmr0 FMR),
+								<<SIM: _hpsim hpsim true f_tgt (st_src, k_src tt) (st_tgt, i_tgt) fmr0>> /\
+								<<IH: P true f_tgt (st_src, k_src tt) (st_tgt, i_tgt) fmr0>>),
+						P f_src f_tgt (st_src, trigger (Guarantee iP) >>= k_src) (st_tgt, i_tgt) fmr)
+				(GUARANTEETGT: forall
+						f_src f_tgt st_src st_tgt fmr
+						iP i_src k_tgt FMR
+						(CUR: current_iProp fmr FMR)
+						(K: forall fmr0 (NEW: current_iProp fmr0 (iP ** FMR)),
+								<<SIM: _hpsim hpsim f_src true (st_src, i_src) (st_tgt, k_tgt tt) fmr0>> /\
+								<<IH: P f_src true (st_src, i_src) (st_tgt, k_tgt tt) fmr0>>),
+						P f_src f_tgt (st_src, i_src) (st_tgt, trigger (Guarantee iP) >>= k_tgt) fmr)
+				(PROGRESS: forall
+						st_src st_tgt fmr
+						i_src i_tgt
+						(SIM: hpsim false false (st_src, i_src) (st_tgt, i_tgt) fmr),
+						P true true (st_src, i_src) (st_tgt, i_tgt) fmr)
+		:		
+		forall f_src f_tgt st_src st_tgt fmr
+		(SIM: @_hpsim hpsim f_src f_tgt st_src st_tgt fmr),
+		P f_src f_tgt st_src st_tgt fmr.
+		Proof.
+			i. induction SIM.
+		{ eapply RET; eauto. }
+		{ eapply CALL; esplits; et. }
+		{ eapply SYSCALL; eauto. }
+		{ eapply INLINESRC; eauto. }
+		{ eapply INLINETGT; eauto. }
+		{ eapply TAUSRC; eauto. }
+		{ eapply TAUTGT; eauto. }
+		{ eapply CHOOSESRC; eauto. }
+		{ eapply CHOOSETGT; eauto. }
+		{ eapply TAKESRC; eauto. }
+		{ eapply TAKETGT; eauto. }
+		{ eapply SUPDATESRC; eauto. }
+		{ eapply SUPDATETGT; eauto. }
+		{ eapply ASSUMESRC; esplits; et. }
+		{ eapply ASSUMETGT; esplits; et. }
+		{ eapply GUARANTEESRC; esplits; et. }
+		{ eapply GUARANTEETGT; esplits; et. }
+		{ eapply PROGRESS; eauto. }
+		Qed.
 
-	Definition hp_sim := paco5 _hpsim bot5.
+		Definition hpsim := paco5 _hpsim bot5.
+
+
+		Lemma _hpsim_mon: monotone5 _hpsim.
+		Proof. 
+			ii. induction IN using _hpsim_ind2;
+			try (econs; et; ii; exploit K; i; des; et).
+		Qed.
+	
+		Hint Constructors _hpsim.
+		Hint Unfold hpsim.
+		Hint Resolve _hpsim_mon: paco.
+		Hint Resolve cpn5_wcompat: paco.
+
+
+		Lemma hpsim_ind
+				(P: bool -> bool -> Any.t * itree hAGEs Any.t -> Any.t * itree hAGEs Any.t -> Σ -> Prop)
+		
+		(RET: forall
+				f_src f_tgt st_src st_tgt fmr
+				v_src v_tgt
+				(RET: current_iProp fmr (I st_src st_tgt)),
+				P f_src f_tgt (st_src, Ret v_src) (st_tgt, Ret v_tgt) fmr)
+		(CALL: forall
+				f_src f_tgt st_src st_tgt fmr
+				fn varg k_src k_tgt FR
+				(INV: current_iProp fmr (I st_src st_tgt ** FR))
+				(K: forall vret st_src0 st_tgt0 fmr0
+						(INV: current_iProp fmr0 (I st_src0 st_tgt0 ** FR)),
+						<<SIM: hpsim true true (st_src0, k_src vret) (st_tgt0, k_tgt vret) fmr0>> /\
+						<<IH: P true true (st_src0, k_src vret) (st_tgt0, k_tgt vret) fmr0>>),
+				P f_src f_tgt (st_src, trigger (Call fn varg) >>= k_src) (st_tgt, trigger (Call fn varg) >>= k_tgt) fmr)
+		(SYSCALL: forall
+				f_src f_tgt st_src st_tgt fmr
+				fn varg rvs k_src k_tgt
+				(K: forall vret,
+						<<SIM: hpsim true true (st_src, k_src vret) (st_tgt, k_tgt vret) fmr>> /\ 
+						<<IH: P true true (st_src, k_src vret) (st_tgt, k_tgt vret) fmr>>),
+				P f_src f_tgt (st_src, trigger (Syscall fn varg rvs) >>= k_src) (st_tgt, trigger (Syscall fn varg rvs) >>= k_tgt) fmr)
+		(INLINESRC: forall
+				f_src f_tgt st_src st_tgt fmr
+				fn f varg k_src i_tgt
+				(FUN: alist_find fn fl_src = Some f)
+				(K: hpsim  true f_tgt (st_src, (f varg) >>= k_src) (st_tgt, i_tgt) fmr)
+				(IH: P true f_tgt (st_src, (f varg) >>= k_src) (st_tgt, i_tgt) fmr),
+				P f_src f_tgt (st_src, trigger (Call fn varg) >>= k_src) (st_tgt, i_tgt) fmr)
+		(INLINETGT: forall
+				f_src f_tgt st_src st_tgt fmr
+				fn f varg i_src k_tgt
+				(FUN: alist_find fn fl_tgt = Some f)
+				(K: hpsim f_src true (st_src, i_src) (st_tgt, (f varg) >>= k_tgt) fmr)
+				(IH: P f_src true (st_src, i_src) (st_tgt, (f varg) >>= k_tgt) fmr),
+				P f_src f_tgt (st_src, i_src) (st_tgt, trigger (Call fn varg) >>= k_tgt) fmr)
+		(TAUSRC: forall
+				f_src f_tgt st_src st_tgt fmr
+				i_src i_tgt
+				(K: hpsim true f_tgt (st_src, i_src) (st_tgt, i_tgt) fmr)
+				(IH: P true f_tgt (st_src, i_src) (st_tgt, i_tgt) fmr),
+				P f_src f_tgt (st_src, tau;; i_src) (st_tgt, i_tgt) fmr)
+		(TAUTGT: forall
+				f_src f_tgt st_src st_tgt fmr
+				i_src i_tgt
+				(K: hpsim f_src true (st_src, i_src) (st_tgt, i_tgt) fmr)
+				(IH: P f_src true (st_src, i_src) (st_tgt, i_tgt) fmr),
+				P f_src f_tgt (st_src, i_src) (st_tgt, tau;; i_tgt) fmr)
+		(CHOOSESRC: forall
+				f_src f_tgt st_src st_tgt fmr
+				X x k_src i_tgt
+				(K: hpsim true f_tgt (st_src, k_src x) (st_tgt, i_tgt) fmr)
+				(IH: P true f_tgt (st_src, k_src x) (st_tgt, i_tgt) fmr),
+				P f_src f_tgt (st_src, trigger (Choose X) >>= k_src) (st_tgt, i_tgt) fmr)
+		(CHOOSETGT: forall
+				f_src f_tgt st_src st_tgt fmr
+				X i_src k_tgt
+				(K: forall (x: X), 
+						<<SIM: hpsim f_src true (st_src, i_src) (st_tgt, k_tgt x) fmr>> /\
+						<<IH: P f_src true (st_src, i_src) (st_tgt, k_tgt x) fmr>>),
+				P f_src f_tgt (st_src, i_src) (st_tgt, trigger (Choose X) >>= k_tgt) fmr)
+		(TAKESRC: forall
+				f_src f_tgt st_src st_tgt fmr
+				X k_src i_tgt
+				(K: forall (x: X), 
+						<<SIM: hpsim true f_tgt (st_src, k_src x) (st_tgt, i_tgt) fmr>> /\
+						<<IH: P true f_tgt (st_src, k_src x) (st_tgt, i_tgt) fmr>>),
+				P f_src f_tgt (st_src, trigger (Take X) >>= k_src) (st_tgt, i_tgt) fmr)
+		(TAKETGT: forall
+				f_src f_tgt st_src st_tgt fmr
+				X x i_src k_tgt
+				(K: hpsim f_src true (st_src, i_src) (st_tgt, k_tgt x) fmr)
+				(IH: P f_src true (st_src, i_src) (st_tgt, k_tgt x) fmr),
+				P f_src f_tgt (st_src, i_src) (st_tgt, trigger (Take X) >>= k_tgt) fmr)
+		(SUPDATESRC: forall
+				f_src f_tgt st_src st_tgt fmr
+				X x st_src0 k_src i_tgt
+				(run: Any.t -> Any.t * X)
+				(RUN: run st_src = (st_src0, x))
+				(K: hpsim true f_tgt (st_src0, k_src x) (st_tgt, i_tgt) fmr)
+				(IH: P true f_tgt (st_src0, k_src x) (st_tgt, i_tgt) fmr),
+				P f_src f_tgt (st_src, trigger (SUpdate run) >>= k_src) (st_tgt, i_tgt) fmr)
+		(SUPDATETGT: forall
+				f_src f_tgt st_src st_tgt fmr
+				X x st_tgt0 i_src k_tgt
+				(run: Any.t -> Any.t * X)
+				(RUN: run st_tgt = (st_tgt0, x))
+				(K: hpsim f_src true (st_src, i_src) (st_tgt0, k_tgt x) fmr)
+				(IH: P f_src true (st_src, i_src) (st_tgt0, k_tgt x) fmr),
+				P f_src f_tgt (st_src, i_src) (st_tgt, trigger (SUpdate run) >>= k_tgt) fmr)
+		(ASSUMESRC: forall
+				f_src f_tgt st_src st_tgt fmr
+				iP k_src i_tgt FMR
+				(CUR: current_iProp fmr FMR)
+				(K: forall fmr0 (NEW: current_iProp fmr0 (iP ** FMR)),
+						<<SIM: hpsim true f_tgt (st_src, k_src tt) (st_tgt, i_tgt) fmr0>> /\
+						<<IH: P true f_tgt (st_src, k_src tt) (st_tgt, i_tgt) fmr0>>),
+				P f_src f_tgt (st_src, trigger (Assume iP) >>= k_src) (st_tgt, i_tgt) fmr)
+		(ASSUMETGT: forall
+				f_src f_tgt st_src st_tgt fmr
+				iP i_src k_tgt FMR
+				(CUR: current_iProp fmr (iP ** FMR))
+				(K: forall fmr0 (NEW: current_iProp fmr0 FMR),
+						<<SIM: hpsim f_src true (st_src, i_src) (st_tgt, k_tgt tt) fmr0>> /\
+						<<IH: P f_src true (st_src, i_src) (st_tgt, k_tgt tt) fmr0>>),
+				P f_src f_tgt (st_src, i_src) (st_tgt, trigger (Assume iP) >>= k_tgt) fmr)
+		(GUARANTEESRC: forall
+				f_src f_tgt st_src st_tgt fmr
+				iP k_src i_tgt FMR
+				(CUR: current_iProp fmr (iP ** FMR))
+				(K: forall fmr0 (NEW: current_iProp fmr0 FMR),
+						<<SIM: hpsim true f_tgt (st_src, k_src tt) (st_tgt, i_tgt) fmr0>> /\
+						<<IH: P true f_tgt (st_src, k_src tt) (st_tgt, i_tgt) fmr0>>),
+				P f_src f_tgt (st_src, trigger (Guarantee iP) >>= k_src) (st_tgt, i_tgt) fmr)
+		(GUARANTEETGT: forall
+				f_src f_tgt st_src st_tgt fmr
+				iP i_src k_tgt FMR
+				(CUR: current_iProp fmr FMR)
+				(K: forall fmr0 (NEW: current_iProp fmr0 (iP ** FMR)),
+						<<SIM: hpsim f_src true (st_src, i_src) (st_tgt, k_tgt tt) fmr0>> /\
+						<<IH: P f_src true (st_src, i_src) (st_tgt, k_tgt tt) fmr0>>),
+				P f_src f_tgt (st_src, i_src) (st_tgt, trigger (Guarantee iP) >>= k_tgt) fmr)
+		(PROGRESS: forall
+				st_src st_tgt fmr
+				i_src i_tgt
+				(SIM: hpsim false false (st_src, i_src) (st_tgt, i_tgt) fmr),
+				P true true (st_src, i_src) (st_tgt, i_tgt) fmr)
+		:
+				forall f_src f_tgt st_src st_tgt fmr
+				(SIM: hpsim f_src f_tgt st_src st_tgt fmr),
+				P f_src f_tgt st_src st_tgt fmr.
+	Proof. 
+    i. punfold SIM. induction SIM using _hpsim_ind2.
+			{ eapply RET; eauto. }
+			{ eapply CALL; eauto. i. hexploit K; et. i. des. esplits; et. }
+			{ eapply SYSCALL; eauto. i. hexploit K; et. i. des. esplits; et. }
+			{ eapply INLINESRC; eauto. }
+			{ eapply INLINETGT; eauto. }
+			{ eapply TAUSRC; eauto. }
+			{ eapply TAUTGT; eauto. }
+			{ eapply CHOOSESRC; eauto. }
+			{ eapply CHOOSETGT; eauto. i. hexploit K; et. i. des. esplits; et. }
+			{ eapply TAKESRC; eauto. i. hexploit K; et. i. des. esplits; et. }
+			{ eapply TAKETGT; eauto. }
+			{ eapply SUPDATESRC; eauto. }
+			{ eapply SUPDATETGT; eauto. }
+			{ eapply ASSUMESRC; eauto. i. hexploit K; et. i. des. esplits; et. }
+			{ eapply ASSUMETGT; eauto. i. hexploit K; et. i. des. esplits; et. }
+			{ eapply GUARANTEESRC; eauto. i. hexploit K; et. i. des. esplits; et. }
+			{ eapply GUARANTEETGT; eauto. i. hexploit K; et. i. des. esplits; et. }
+			{ eapply PROGRESS; eauto. pclearbot. et. }
+	Qed.
+
+  Variant mk_inv  
+          (I: Any.t -> Any.t -> iProp)
+    : unit -> Any.t * Any.t -> Prop :=
+  | mk_inv_intro
+      mr_src st_src mr_tgt st_tgt
+      (INV: 
+						(* forall (WF: URA.wf mr_src),  *)
+						exists MR_tgt,
+						<<MRS: current_iProp mr_src (I st_src st_tgt ** MR_tgt)>> /\
+						<<MRT: current_iProp mr_tgt MR_tgt>>)
+    :
+      mk_inv I tt (Any.pair st_src mr_src↑, Any.pair st_tgt mr_tgt↑)
+  .
+
+	(* Check _sim_itree. *)
+
+
+  Lemma hpsim_adequacy:
+    forall
+      f_src f_tgt st_src st_tgt fl_src fl_tgt itr_src itr_tgt
+			(mr_src mr_tgt fr_src fr_tgt: Σ) FR FR_tgt
+      (SIM: hpsim f_src f_tgt (st_src, itr_src) (st_tgt, itr_tgt) (fr_src ⋅ mr_src))
+			(FRS: current_iProp fr_src (FR ** FR_tgt))
+			(FRT: current_iProp fr_tgt FR_tgt),
+
+			@sim_itree unit (mk_inv I) (fun _ _ => True) fl_src fl_tgt f_src f_tgt tt 
+			(Any.pair st_src mr_src↑, (interp_hp_tgt itr_src fr_src) >>= (fun r => Ret (snd r)))
+			(Any.pair st_tgt mr_tgt↑, (interp_hp_tgt itr_tgt fr_tgt) >>= (fun r => Ret (snd r))).
+  Proof.
+		i. 
+		remember (Any.pair st_src mr_src↑). remember (Any.pair st_tgt mr_tgt↑).
+		revert_until I.
+		ginit. gcofix CIH. i.
+		remember (st_src, itr_src). remember (st_tgt, itr_tgt).
+		
+		revert st_src st_tgt itr_src itr_tgt Heqp Heqp0 Heqt Heqt0 CIH.
+		induction SIM using hpsim_ind; i; clarify.
+		- steps. econs; esplits; et. admit. admit.
+		- steps. { admit. } hexploit K; et. i. des. eapply IH.
+	Admitted.
 
 
 
 
+
+
+
+
+	(* Variable fl_src: alist gname (Any.t -> itree hAGEs Any.t).
+	Variable fl_tgt: alist gname (Any.t -> itree hAGEs Any.t).
+	Variable I: Any.t -> Any.t -> iProp.
+  Variable Any.t Any.t: Type.
+  Variable Q: Any.t -> Any.t -> Any.t -> Any.t -> iProp.
+  (* Variable Q: Any.t -> Any.t -> Prop. *)
+  
+  (* Print iProp.
+  Print URA.t. *)
+	(* Print current_iProp. *)
+
+	Inductive _hpsim
+	(hpsim: bool -> bool -> Any.t * itree hAGEs Any.t -> Any.t * itree hAGEs Any.t -> Σ -> Prop)
+		: bool -> bool -> Any.t * itree hAGEs Any.t -> Any.t * itree hAGEs Any.t -> Σ -> Prop :=
+	| hpsim_ret *)
 
 	(****** ******)
 
 	(* Inductive _hpsim
-	(hpsim: bool -> bool -> (Any.t * Σ) * itree hAGEs R_src -> (Any.t * Σ) * itree hAGEs R_tgt -> Σ -> Prop)
-		: bool -> bool -> (Any.t * Σ) * itree hAGEs R_src -> (Any.t * Σ) * itree hAGEs R_tgt -> Σ -> Prop :=
+	(hpsim: bool -> bool -> (Any.t * Σ) * itree hAGEs Any.t -> (Any.t * Σ) * itree hAGEs Any.t -> Σ -> Prop)
+		: bool -> bool -> (Any.t * Σ) * itree hAGEs Any.t -> (Any.t * Σ) * itree hAGEs Any.t -> Σ -> Prop :=
 	| hpsim_ret
 			f_src f_tgt st_src st_tgt mr_src mr_tgt fr
 			v_src v_tgt
@@ -310,32 +693,32 @@ Section SIM.
 
 	| hpsim_assume_src
 			f_src f_tgt st_src st_tgt mr_src mr_tgt fr
-			P k_src i_tgt r 
-      (ASM: current_iProp r P)
+			iP k_src i_tgt r 
+      (ASM: current_iProp r iP)
 			(K: _hpsim hpsim true f_tgt ((st_src, mr_src), k_src tt) ((st_tgt, mr_tgt), i_tgt) fr)
 		:
-			_hpsim hpsim f_src f_tgt ((st_src, mr_src), trigger (Assume P) >>= k_src) ((st_tgt, mr_tgt), i_tgt) fr
+			_hpsim hpsim f_src f_tgt ((st_src, mr_src), trigger (Assume iP) >>= k_src) ((st_tgt, mr_tgt), i_tgt) fr
 
 	| hpsim_assume_tgt
 			f_src f_tgt st_src st_tgt mr_src mr_tgt fr
 			f_src f_tgt st_src st_tgt i_src k_tgt
-			(K: (P ** (_hpsim hpsim f_src true ((st_src, mr_src), i_src) ((st_tgt, mr_tgt), k_tgt tt))) fr)
+			(K: (iP ** (_hpsim hpsim f_src true ((st_src, mr_src), i_src) ((st_tgt, mr_tgt), k_tgt tt))) fr)
 		:
-			_hpsim hpsim f_src f_tgt ((st_src, mr_src), i_src) ((st_tgt, mr_tgt), trigger (Assume P) >>= k_tgt) fr
+			_hpsim hpsim f_src f_tgt ((st_src, mr_src), i_src) ((st_tgt, mr_tgt), trigger (Assume iP) >>= k_tgt) fr
 
 	| hpsim_guarantee_src
-			P fr
+			iP fr
 			f_src f_tgt st_src st_tgt k_src i_tgt
-			(K: (P ** (_hpsim hpsim true f_tgt ((st_src, mr_src), k_src tt) ((st_tgt, mr_tgt), i_tgt))) fr)
+			(K: (iP ** (_hpsim hpsim true f_tgt ((st_src, mr_src), k_src tt) ((st_tgt, mr_tgt), i_tgt))) fr)
 		:
-			_hpsim hpsim f_src f_tgt ((st_src, mr_src), trigger (Guarantee P) >>= k_src) ((st_tgt, mr_tgt), i_tgt) fr
+			_hpsim hpsim f_src f_tgt ((st_src, mr_src), trigger (Guarantee iP) >>= k_src) ((st_tgt, mr_tgt), i_tgt) fr
 
 	| hpsim_guarantee_tgt
-			P fr
+			iP fr
 			f_src f_tgt st_src st_tgt i_src k_tgt
-			(K: (P -* (_hpsim hpsim f_src true ((st_src, mr_src), i_src) ((st_tgt, mr_tgt), k_tgt tt))) fr)
+			(K: (iP -* (_hpsim hpsim f_src true ((st_src, mr_src), i_src) ((st_tgt, mr_tgt), k_tgt tt))) fr)
 		:
-			_hpsim hpsim f_src f_tgt ((st_src, mr_src), i_src) ((st_tgt, mr_tgt), trigger (Guarantee P) >>= k_tgt) fr
+			_hpsim hpsim f_src f_tgt ((st_src, mr_src), i_src) ((st_tgt, mr_tgt), trigger (Guarantee iP) >>= k_tgt) fr
 
 	| hpsim_progress
 		fr
